ironfleet/src/Dafny/Distributed/Impl/Lock/Node.i.dfy
@@ -24,7 +24,7 @@ predicate ValidConfig(c:Config)
 
 predicate ValidConfigIndex(c:Config, index:uint64)
 {
-    0 <= int(index) < |c|
+    0 <= index as int < |c|
 }
 
 predicate CNodeValid(c:CNode)
@@ -35,15 +35,15 @@ predicate CNodeValid(c:CNode)
 
 function AbstractifyCNode(n:CNode) : Node
 {
-    Node(n.held, int(n.epoch), int(n.my_index), n.config)
+    Node(n.held, n.epoch as int, n.my_index as int, n.config)
 }
 
 method NodeInitImpl(my_index:uint64, config:Config) returns (node:CNode)
     requires 0 < |config| < 0x1_0000_0000_0000_0000;
-    requires 0 <= int(my_index) < |config|;
+    requires 0 <= my_index as int < |config|;
     requires ValidConfig(config);
     ensures CNodeValid(node);
-    ensures NodeInit(AbstractifyCNode(node), int(my_index), config);
+    ensures NodeInit(AbstractifyCNode(node), my_index as int, config);
     ensures node.my_index == my_index;
     ensures node.config == config;
 {
