ironfleet/src/Dafny/Distributed/Common/Framework/EnvironmentTCP.s.dfy
@@ -1,0 +1,254 @@
+include "../Collections/Maps2.s.dfy"
+include "../Logic/Temporal/Temporal.s.dfy"
+
+module EnvironmentTCP_s {
+import opened Collections__Maps2_s
+import opened Temporal__Temporal_s
+
+
+/*****************************************************************************************
+*                                        Types                                           *
+******************************************************************************************/   
+
+datatype LPacket<IdType, MessageType(==)> = LPacket(dst:IdType, src:IdType, sender_index:int, msg:MessageType)
+
+datatype LIoOp<IdType, MessageType(==)> = LIoOpSend(s:LPacket<IdType, MessageType>)
+                                        | LIoOpReceive(r:LPacket<IdType, MessageType>)
+                                        | LIoOpTimeoutReceive()
+                                        | LIoOpReadClock(t:int)
+
+datatype LEnvStep<IdType, MessageType(==)> = LEnvStepHostIos(actor:IdType, ios:seq<LIoOp<IdType, MessageType>>)
+                                           | LEnvStepDeliverPacket(p:LPacket<IdType, MessageType>)
+                                           | LEnvStepAdvanceTime()
+                                           | LEnvStepStutter()
+
+datatype LHostInfo<IdType, MessageType(==)> = LHostInfo(queue:seq<LPacket<IdType, MessageType>>)
+
+// Channel[..i] are the delievered prefix
+datatype HostChannel<IdType, MessageType> = HostChannel(index:int, channel:seq<LPacket<IdType, MessageType>>)
+
+datatype LEnvironment<IdType, MessageType(==)> = LEnvironment(time:int,
+                                                              config:seq<IdType>,
+                                                              channels:map<IdType, HostChannel<IdType, MessageType>>,
+                                                              ghost sentPackets:set<LPacket<IdType, MessageType>>,
+                                                              hostInfo:map<IdType, LHostInfo<IdType, MessageType>>,
+                                                              nextStep:LEnvStep<IdType, MessageType>)
+
+/*****************************************************************************************
+*                                     Validity Checks                                    *
+******************************************************************************************/                                        
+predicate IsValidLIoOp<IdType, MessageType>(io:LIoOp, actor:IdType, e:LEnvironment<IdType, MessageType>)
+{
+    match io
+        case LIoOpSend(s) => s.src == actor && s.src in e.config && s.dst in e.config
+        case LIoOpReceive(r) => r.dst == actor && r.src in e.config && r.dst in e.config
+        case LIoOpTimeoutReceive => true
+        case LIoOpReadClock(t) => true
+}
+
+predicate LIoOpOrderingOKForAction<IdType, MessageType>(
+    io1:LIoOp<IdType, MessageType>,
+    io2:LIoOp<IdType, MessageType>
+    )
+{
+    io1.LIoOpReceive? || io2.LIoOpSend?
+}
+
+predicate LIoOpSeqCompatibleWithReduction<IdType, MessageType>(
+    ios:seq<LIoOp<IdType, MessageType>>
+    )
+{
+    forall i {:trigger ios[i], ios[i+1]} :: 0 <= i < |ios| - 1 ==> LIoOpOrderingOKForAction(ios[i], ios[i+1])
+}
+
+/* Returns true iff s1 is a prefix of s2 */
+predicate IsPrefix<T>(s1: seq<T>, s2: seq<T>) {
+    && |s1| <= |s2|
+    && s2[0..|s1|] == s2
+}
+
+predicate IsValidReceiveSeq<IdType, MessageType>(rcvSeq:seq<LPacket<IdType, MessageType>>, hc:HostChannel) 
+{
+    && 0 <= hc.index <= |hc.channel|
+    && IsPrefix(rcvSeq, hc.channel[hc.index..])
+}
+
+predicate IsValidLEnvStep<IdType, MessageType>(e:LEnvironment<IdType, MessageType>, step:LEnvStep)
+{
+    match step
+        case LEnvStepHostIos(actor, ios) =>    
+            var rcvMap := IosToRcvMap(ios);
+            && (forall io :: io in ios ==> IsValidLIoOp(io, actor, e))
+            && (forall receiver | receiver in rcvMap :: receiver in e.channels && IsValidReceiveSeq(rcvMap[receiver], e.channels[receiver]))
+            && LIoOpSeqCompatibleWithReduction(ios)
+        case LEnvStepDeliverPacket(p) => p.dst in e.channels && p in e.channels[p.dst].channel
+        case LEnvStepAdvanceTime => true
+        case LEnvStepStutter => true
+}
+
+
+/*****************************************************************************************
+*                                       Actions                                          *
+******************************************************************************************/ 
+
+
+/* Transform a seq of IoOps to a map that maps each dst to a sequence of send ops to that dst*/
+function IosToSendMap<IdType, MessageType>(ios:seq<LIoOp<IdType, MessageType>>) : map<IdType, seq<LPacket<IdType, MessageType>>> {
+    if |ios| == 0 then map[]
+    else 
+        var head := ios[0];
+        var sub_map := IosToSendMap(ios[1..]);
+        if head.LIoOpSend? then (
+            if head.s.dst in sub_map then sub_map[head.s.dst := sub_map[head.s.dst] + [head.s]]
+            else sub_map[head.s.dst := [head.s]]
+        ) else sub_map
+}
+
+/* Transform a seq of IoOps to a map that maps each dst to a sequence of receive ops to that dst
+* Note that IsValidLIoOp ensures that for a valid ios seq, the resulting map has exactly one
+* key which is the actor */
+function IosToRcvMap<IdType, MessageType>(ios:seq<LIoOp<IdType, MessageType>>) : map<IdType, seq<LPacket<IdType, MessageType>>> {
+    if |ios| == 0 then map[]
+    else 
+        var head := ios[0];
+        var sub_map := IosToRcvMap(ios[1..]);
+        if head.LIoOpReceive? then (
+            if head.r.dst in sub_map then sub_map[head.r.dst := sub_map[head.r.dst] + [head.r]]
+            else sub_map[head.r.dst := [head.r]]
+        ) else sub_map
+}
+
+
+predicate LEnvironment_Init<IdType, MessageType>(
+    config:seq<IdType>,
+    e:LEnvironment<IdType, MessageType>)
+{
+    && (forall h | h in config :: h in e.channels && e.channels[h] == HostChannel(0, []))
+    && e.config == config
+    && e.sentPackets == {}
+    && e.time >= 0
+}
+
+
+/* Maps channels to its new state after a sending and receiving a set of ios in sendMap
+* and rcvMap */
+function PerformIos<IdType, MessageType>(
+    channels:map<IdType, HostChannel>, 
+    sendMap: map<IdType, seq<LPacket<IdType, MessageType>>>,
+    rcvMap: map<IdType, seq<LPacket<IdType, MessageType>>>) :
+    map<IdType, HostChannel>
+{
+    map h | h in channels :: (
+        if h in rcvMap then (
+            if h in sendMap 
+                then HostChannel(channels[h].index + |rcvMap[h]|, channels[h].channel + sendMap[h])
+                else HostChannel(channels[h].index + |rcvMap[h]|, channels[h].channel)
+        ) else (
+            if h in sendMap 
+                then HostChannel(channels[h].index, channels[h].channel + sendMap[h])
+                else channels[h]
+        )
+    )
+}
+
+
+predicate LEnvironment_PerformIos<IdType, MessageType>(
+    e:LEnvironment<IdType, MessageType>,
+    e':LEnvironment<IdType, MessageType>,
+    actor:IdType,
+    ios:seq<LIoOp<IdType, MessageType>>
+    )
+{
+    var sendMap := IosToSendMap(ios);
+    var rcvMap := IosToRcvMap(ios);
+    && (forall io :: io in ios && io.LIoOpReceive? ==> io.r in e.sentPackets)
+    && e'.channels == PerformIos(e.channels, sendMap, rcvMap)
+    && e'.sentPackets == e.sentPackets + (set io | io in ios && io.LIoOpSend? :: io.s)
+    && e'.time == e.time
+}
+
+predicate LEnvironment_AdvanceTime<IdType, MessageType>(
+    e:LEnvironment<IdType, MessageType>,
+    e':LEnvironment<IdType, MessageType>
+    )
+{
+       e'.time > e.time
+    // UNCHANGED
+    && e'.channels == e.channels
+}
+
+predicate LEnvironment_Stutter<IdType, MessageType>(
+    e:LEnvironment<IdType, MessageType>,
+    e':LEnvironment<IdType, MessageType>
+    )
+{
+       e'.time == e.time
+    && e'.channels == e.channels
+}
+
+predicate LEnvironment_Next<IdType, MessageType>(
+    e:LEnvironment<IdType, MessageType>,
+    e':LEnvironment<IdType, MessageType>
+    )
+{
+       IsValidLEnvStep(e, e.nextStep)
+    && e'.config == e.config
+    && match e.nextStep
+           case LEnvStepHostIos(actor, ios) => LEnvironment_PerformIos(e, e', actor, ios)
+           case LEnvStepDeliverPacket(p) => LEnvironment_Stutter(e, e') // this is only relevant for synchrony
+           case LEnvStepAdvanceTime => LEnvironment_AdvanceTime(e, e')
+           case LEnvStepStutter => LEnvironment_Stutter(e, e')
+}
+
+
+
+/*****************************************************************************************
+*                                     Utilities                                          *
+******************************************************************************************/ 
+
+/* Creates a set containing exactly all the messages in channels map */
+function ChannelsToSet<IdType, MessageType>(channels:map<IdType, HostChannel<IdType, MessageType>>) : set<LPacket<IdType, MessageType>> 
+    decreases channels
+    ensures forall ep | ep in channels :: (
+    forall pkt | pkt in channels[ep].channel :: pkt in ChannelsToSet(channels)
+    );
+    ensures forall pkt | pkt in ChannelsToSet(channels) ::
+        exists e :: e in channels && pkt in channels[e].channel
+{
+    if |channels| == 0 then {}
+    else 
+        var ep :| ep in channels;
+        var remaining_channels := map e | e in channels && e != ep :: channels[e];
+        var curr_set := (set pkt | pkt in channels[ep].channel :: pkt);
+        var rem_set := ChannelsToSet(remaining_channels);
+        assert forall e | e in channels :: (
+            forall pkt | pkt in channels[e].channel ::
+                if e == ep then pkt in curr_set else e in remaining_channels && pkt in rem_set
+        );
+        curr_set + rem_set
+}
+
+
+/*****************************************************************************************
+*                                     Temporals                                          *
+******************************************************************************************/ 
+
+
+// function{:opaque} EnvironmentNextTemporal<IdType, MessageType, NodeStepType>(b:Behavior<LEnvironment<IdType, MessageType, NodeStepType>>):temporal
+//     requires imaptotal(b);
+//     ensures forall i {:trigger sat(i, EnvironmentNextTemporal(b))} ::
+//                 sat(i, EnvironmentNextTemporal(b)) <==> LEnvironment_Next(b[i], b[i+1]);
+// {
+//     stepmap(imap i :: LEnvironment_Next(b[i], b[i+1]))
+// }
+
+// predicate LEnvironment_BehaviorSatisfiesSpec<IdType, MessageType, NodeStepType>(
+//     b:Behavior<LEnvironment<IdType, MessageType, NodeStepType>>
+//     )
+// {
+//        imaptotal(b)
+//     && LEnvironment_Init(b[0])
+//     && sat(0, always(EnvironmentNextTemporal(b)))
+// }
+
+} 
