ironfleet/src/Dafny/Distributed/Protocol/Lock/PerformanceProof/Invariants.i.dfy
@@ -1,0 +1,406 @@
+include "../../../Common/Framework/Environment.s.dfy"
+include "TimestampedGLS.i.dfy"
+
+module Invariants_i {
+    import opened TimestampedGLS_i
+    import opened Environment_s
+
+
+/*****************************************************************************************
+/                           ValidBehavior translation lemma                              *
+*****************************************************************************************/
+
+lemma lemma_ValidBehavior(config:Config, tglb:seq<TimestampedGLS_State>) 
+    requires |config| > 1;
+    requires ValidTimestampedGLSBehavior(tglb, config);
+    ensures forall i | 0 <= i < |tglb| - 1 :: TGLS_Next(tglb[i], tglb[i+1]);
+{
+    forall i | 0 <= i < |tglb| - 1
+    ensures TGLS_Next(tglb[i], tglb[i+1]) {
+        var h' := i + 1;
+        var h := h' - 1;
+        assert 0 <= h < h' < |tglb|;
+        assert TGLS_Next(tglb[h], tglb[h']);
+    }
+}
+
+
+
+/*****************************************************************************************
+/                                 ConfigurationInvariant                                 *
+*****************************************************************************************/
+
+
+/* Invariants about servers in gls and the config */
+predicate {:opaque} ConfigInvariant(config:ConcreteConfiguration, tgls:TimestampedGLS_State) 
+{
+    && tgls.tls.config == config
+    && (forall ep :: ep in tgls.tls.t_servers <==> ep in config)
+    && (forall ep | ep in tgls.tls.t_servers :: tgls.tls.t_servers[ep].v.config == config)
+    && (forall ep | ep in tgls.tls.t_servers :: 0 <= tgls.tls.t_servers[ep].v.my_index < |config|)
+    && (forall ep | ep in tgls.tls.t_servers :: ep == config[tgls.tls.t_servers[ep].v.my_index])
+}
+
+lemma lemma_ConfigInvariant(config:ConcreteConfiguration, tglb:seq<TimestampedGLS_State>) 
+    requires |config| > 1;
+    requires ValidTimestampedGLSBehavior(tglb, config)
+    ensures forall i | 0 <= i < |tglb| :: ConfigInvariant(config, tglb[i]);
+{
+    reveal_ConfigInvariant();
+    lemma_ValidBehavior(config, tglb);
+    var ls := UntagLS_State(tglb[0].tls);
+    assert LS_Init(ls, config);
+    assert forall e :: e in config <==> e in ls.servers;
+    assert forall ep | ep in ls.servers :: ls.servers[ep].config == config;
+    assert ConfigInvariant(config, tglb[0]);
+
+    var i := 0;
+    while i < |tglb| - 1
+        decreases |tglb| - i;
+        invariant 0 <= i < |tglb|;
+        invariant forall k | 0 <= k <= i :: ConfigInvariant(config, tglb[k]);
+    {
+        var tgls, tgls' := tglb[i], tglb[i+1];
+        assert TGLS_Next(tgls, tgls');
+        assert forall ep :: ep in tgls'.tls.t_servers <==> ep in tgls.tls.t_servers;
+        assert forall ep | ep in tgls'.tls.t_servers :: tgls'.tls.t_servers[ep].v.config == tgls.tls.t_servers[ep].v.config;
+        assert forall ep | ep in tgls'.tls.t_servers :: tgls'.tls.t_servers[ep].v.my_index == tgls.tls.t_servers[ep].v.my_index;
+        assert ConfigInvariant(config, tglb[i+1]);
+        i := i + 1;    
+    }
+}
+
+
+/*****************************************************************************************
+/                                 HistoryLengthInvariant                                 *
+*****************************************************************************************/
+
+
+predicate HistoryLengthInvariant(config:ConcreteConfiguration, tgls:TimestampedGLS_State)
+    requires |tgls.history| > 0;
+    requires forall ep :: ep in tgls.tls.t_servers <==> ep in config;
+    requires forall ep | ep in tgls.tls.t_servers :: tgls.tls.t_servers[ep].v.config == config;
+{
+    && AtMostOneLockHolder(config, tgls)
+    && NoLockHolderImpliesOneTransferMessageInFlight(config, tgls)
+    && AllTransferMessageInFlightHaveDstLastInHistory(config, tgls)
+    && AllTransferMessageInFlightHaveEpochEqualsHistoryLength(config, tgls)
+    && SomeLockHolderImpliesNoTransferMessageInFlight(config, tgls)
+    && SomeLockHolderImpliesHolderIsLastInHistory(config, tgls)
+    && SomeLockHolderImpliesEpochIsHistoryLength(config, tgls)
+}
+
+
+
+predicate AtMostOneLockHolder(config:ConcreteConfiguration, gls:TimestampedGLS_State) 
+    requires forall ep :: ep in gls.tls.t_servers <==> ep in config;
+    requires forall ep | ep in gls.tls.t_servers :: gls.tls.t_servers[ep].v.config == config;
+{
+    forall ep1, ep2 | ep1 in config && ep2 in config :: gls.tls.t_servers[ep1].v.held && gls.tls.t_servers[ep2].v.held ==> ep1 == ep2
+}   
+
+predicate NoLockHolder(config:ConcreteConfiguration, gls:TimestampedGLS_State) 
+    requires forall ep :: ep in gls.tls.t_servers <==> ep in config;
+    requires forall ep | ep in gls.tls.t_servers :: gls.tls.t_servers[ep].v.config == config;
+{
+    forall ep | ep in config :: !gls.tls.t_servers[ep].v.held
+}
+
+
+predicate IsInFlightTransferMessage(config:ConcreteConfiguration, gls:TimestampedGLS_State, p:LPacket<EndPoint, LockMessage>) 
+    requires forall ep :: ep in gls.tls.t_servers <==> ep in config;
+    requires forall ep | ep in gls.tls.t_servers :: gls.tls.t_servers[ep].v.config == config;
+{
+    && p in UntagSentPkts(gls.tls.t_environment.sentPackets)
+    && p.dst in config 
+    && p.src in config 
+    && p.msg.Transfer?
+    && p.msg.transfer_epoch > gls.tls.t_servers[p.dst].v.epoch
+}
+
+predicate OneTransferMessageIsInFlight(config:ConcreteConfiguration, gls:TimestampedGLS_State) 
+    requires forall ep :: ep in gls.tls.t_servers <==> ep in config;
+    requires forall ep | ep in gls.tls.t_servers :: gls.tls.t_servers[ep].v.config == config;
+{
+    forall p1, p2 | IsInFlightTransferMessage(config, gls, p1) && IsInFlightTransferMessage(config, gls, p2) :: p1 == p2
+}
+
+predicate ZeroTransferMessageIsInFlight(config:ConcreteConfiguration, gls:TimestampedGLS_State) 
+    requires forall ep :: ep in gls.tls.t_servers <==> ep in config;
+    requires forall ep | ep in gls.tls.t_servers :: gls.tls.t_servers[ep].v.config == config;
+{
+    forall p | p in UntagSentPkts(gls.tls.t_environment.sentPackets)  :: ! IsInFlightTransferMessage(config, gls, p)
+}
+
+predicate NoLockHolderImpliesOneTransferMessageInFlight(config:ConcreteConfiguration, gls:TimestampedGLS_State) 
+    requires forall ep :: ep in gls.tls.t_servers <==> ep in config;
+    requires forall ep | ep in gls.tls.t_servers :: gls.tls.t_servers[ep].v.config == config;
+{
+    NoLockHolder(config, gls) ==> OneTransferMessageIsInFlight(config, gls)
+}   
+
+predicate AllTransferMessageInFlightHaveDstLastInHistory(config:ConcreteConfiguration, gls:TimestampedGLS_State)
+    requires |gls.history| > 0;
+    requires forall ep :: ep in gls.tls.t_servers <==> ep in config;
+    requires forall ep | ep in gls.tls.t_servers :: gls.tls.t_servers[ep].v.config == config;
+{
+    forall p | IsInFlightTransferMessage(config, gls, p) :: p.dst == gls.history[|gls.history|-1]
+}   
+
+predicate AllTransferMessageInFlightHaveEpochEqualsHistoryLength(config:ConcreteConfiguration, gls:TimestampedGLS_State)
+    requires |gls.history| > 0;
+    requires forall ep :: ep in gls.tls.t_servers <==> ep in config;
+    requires forall ep | ep in gls.tls.t_servers :: gls.tls.t_servers[ep].v.config == config;
+{
+    forall p | IsInFlightTransferMessage(config, gls, p) :: p.msg.transfer_epoch == |gls.history|
+}   
+
+predicate SomeLockHolderImpliesNoTransferMessageInFlight(config:ConcreteConfiguration, gls:TimestampedGLS_State) 
+    requires forall ep :: ep in gls.tls.t_servers <==> ep in config;
+    requires forall ep | ep in gls.tls.t_servers :: gls.tls.t_servers[ep].v.config == config;
+{
+    !NoLockHolder(config, gls) ==> ZeroTransferMessageIsInFlight(config, gls)
+}   
+
+predicate SomeLockHolderImpliesEpochIsHistoryLength(config:ConcreteConfiguration, gls:TimestampedGLS_State) 
+    requires forall ep :: ep in gls.tls.t_servers <==> ep in config;
+    requires forall ep | ep in gls.tls.t_servers :: gls.tls.t_servers[ep].v.config == config;
+{
+    forall h | h in config && gls.tls.t_servers[h].v.held :: gls.tls.t_servers[h].v.epoch == |gls.history|
+}   
+
+predicate SomeLockHolderImpliesHolderIsLastInHistory(config:ConcreteConfiguration, gls:TimestampedGLS_State)
+    requires |gls.history| > 0;
+    requires forall ep :: ep in gls.tls.t_servers <==> ep in config;
+    requires forall ep | ep in gls.tls.t_servers :: gls.tls.t_servers[ep].v.config == config;
+{
+    forall ep | ep in config && gls.tls.t_servers[ep].v.held :: gls.history[|gls.history|-1] == ep
+}
+
+
+/* Proof of HistoryLengthInvariant */
+lemma lemma_History_Length_Invariant(config:ConcreteConfiguration, tglb:seq<TimestampedGLS_State>)
+    requires |tglb| > 0;
+    requires  TGLS_Init(tglb[0], config);
+    requires forall i {:trigger TGLS_Next(tglb[i], tglb[i+1])} :: 0 <= i < |tglb| - 1 ==>  TGLS_Next(tglb[i], tglb[i+1]);
+    requires forall i | 0 <= i < |tglb| :: (forall ep :: ep in tglb[i].tls.t_servers <==> ep in config);
+    requires forall i | 0 <= i < |tglb| :: (forall ep | ep in tglb[i].tls.t_servers :: tglb[i].tls.t_servers[ep].v.config == config);
+    ensures forall i | 0 <= i < |tglb| :: SomeLockHolderImpliesEpochIsHistoryLength(config, tglb[i]);
+    ensures forall i | 0 <= i < |tglb| :: |tglb[i].history| > 0;
+    ensures forall i | 0 <= i < |tglb| :: HistoryLengthInvariant(config, tglb[i]);
+{
+    // Base Case
+    assert tglb[0].history == [config[0]];
+    assert tglb[0].tls.t_servers[config[0]].v.epoch == 1;
+    assert HistoryLengthInvariant(config, tglb[0]);
+
+    // Inductive Case
+    var i := 1;
+    while i < |tglb| 
+        decreases |tglb| - i;
+        invariant 1 <= i <= |tglb|;
+        invariant forall k | 0 <= k < |tglb|-1 :: TGLS_Next(tglb[k], tglb[k+1]);
+        invariant forall k | 0 <= k < i :: |tglb[k].history| > 0;
+        invariant forall k | 0 <= k < i :: HistoryLengthInvariant(config, tglb[k]);
+    {
+        var k := i-1;
+        var tgls, tgls' := tglb[k], tglb[k+1];
+        assert HistoryLengthInvariant(config, tgls);
+
+        if !NoLockHolder(config, tgls) {
+            // If someone holds the lock in state gls. 
+            // Then I know that there are no Transfer messages in flight in gls
+            lemma_History_Length_Invariant_Induction_A(config, tgls, tgls');
+        } else {
+            // If no one holds the lock in state gls. 
+            // Then I know that there is only one Transfer message in flight in gls
+            assert NoLockHolder(config, tgls);
+            lemma_History_Length_Invariant_Induction_B(config, tgls, tgls');
+        }
+        assert HistoryLengthInvariant(config, tgls');
+        forall k | 0 <= k <= i 
+        ensures HistoryLengthInvariant(config, tglb[k])
+        {}
+        forall k | 0 <= k <= i 
+        ensures |tglb[k].history| > 0
+        {}
+        i := i + 1; 
+    }
+}
+
+/* First branch of lemma_History_Length_Invariant proof, 
+* where !NoLockHolder(config, gls); */
+lemma lemma_History_Length_Invariant_Induction_A(config:ConcreteConfiguration, tgls:TimestampedGLS_State, tgls':TimestampedGLS_State)
+    requires forall ep :: ep in tgls.tls.t_servers <==> ep in config;
+    requires forall ep | ep in tgls.tls.t_servers :: tgls.tls.t_servers[ep].v.config == config;
+    requires TGLS_Next(tgls, tgls');
+    requires |tgls.history| > 0
+    requires HistoryLengthInvariant(config, tgls);
+    requires !NoLockHolder(config, tgls);
+    ensures |tgls'.history| > 0
+    ensures HistoryLengthInvariant(config, tgls');
+{
+    assert ZeroTransferMessageIsInFlight(config, tgls);
+    var gls, gls' := UntagGLS_State(tgls), UntagGLS_State(tgls');
+    assert LS_Next(gls.ls, gls'.ls);
+
+    if (&& gls.ls.environment.nextStep.LEnvStepHostIos? 
+        && gls.ls.environment.nextStep.actor in gls.ls.servers) {
+        // If gls->gls' is a node Grant or Accept step
+        var id, ios := gls.ls.environment.nextStep.actor, gls.ls.environment.nextStep.ios;
+        assert NodeNext(gls.ls.servers[id], gls'.ls.servers[id], ios);
+
+        if NodeGrant(gls.ls.servers[id], gls'.ls.servers[id], ios) {
+            assert HistoryLengthInvariant(config, tgls');  // Dafny magic!
+        } else {
+            assert NodeAccept(gls.ls.servers[id], gls'.ls.servers[id], ios);
+            if ios[0].LIoOpTimeoutReceive? {
+                assert gls'.ls.servers == gls.ls.servers;
+                assert gls'.ls.environment.sentPackets == gls.ls.environment.sentPackets;
+            } else {
+                if (&& !gls.ls.servers[id].held
+                    && ios[0].r.src in gls.ls.servers[id].config
+                    && ios[0].r.msg.Transfer? 
+                    && ios[0].r.msg.transfer_epoch > gls.ls.servers[id].epoch
+                ) {
+                    assert ios[0].LIoOpReceive?;
+                    assert IsValidLIoOp(ios[0], id, gls.ls.environment);
+                    var m := ios[0].r;
+                    assert m in gls.ls.environment.sentPackets;
+                    assert m.dst == id; 
+                    assert false; // contradicts ZeroTransferMessageIsInFlight(config, gls)
+                } else {
+                    assert gls'.ls.servers == gls.ls.servers;
+                    assert gls'.ls.environment.sentPackets == gls.ls.environment.sentPackets;
+                }
+            }
+        }
+        assert HistoryLengthInvariant(config, tgls');
+    } else {
+        // If gls->gls' is purely an environment step
+        assert gls.ls.servers == gls'.ls.servers && gls.history == gls'.history;
+        if !gls.ls.environment.nextStep.LEnvStepHostIos? {
+            match gls.ls.environment.nextStep {
+                case LEnvStepHostIos(actor, ios, nodestep) => assert false;
+                case LEnvStepDeliverPacket(p) => assert LEnvironment_Stutter(gls.ls.environment, gls'.ls.environment);
+                case LEnvStepAdvanceTime => assert LEnvironment_AdvanceTime(gls.ls.environment, gls'.ls.environment);
+                case LEnvStepStutter => assert LEnvironment_Stutter(gls.ls.environment, gls'.ls.environment);
+            }
+            assert gls'.ls.environment.sentPackets == gls.ls.environment.sentPackets;
+        } else {
+            assert gls.ls.environment.nextStep.actor !in gls.ls.servers;
+        }
+        assert HistoryLengthInvariant(config, tgls');
+    }
+}
+
+
+/* Second branch of lemma_History_Length_Invariant proof, 
+* where NoLockHolder(config, gls); */
+lemma lemma_History_Length_Invariant_Induction_B(config:ConcreteConfiguration, tgls:TimestampedGLS_State, tgls':TimestampedGLS_State)
+    requires forall ep :: ep in tgls.tls.t_servers <==> ep in config;
+    requires forall ep | ep in tgls.tls.t_servers :: tgls.tls.t_servers[ep].v.config == config;
+    requires TGLS_Next(tgls, tgls');
+    requires |tgls.history| > 0
+    requires HistoryLengthInvariant(config, tgls);
+    requires NoLockHolder(config, tgls);
+    ensures |tgls'.history| > 0
+    ensures HistoryLengthInvariant(config, tgls');
+{
+    assert OneTransferMessageIsInFlight(config, tgls);
+    var gls, gls' := UntagGLS_State(tgls), UntagGLS_State(tgls');
+    assert LS_Next(gls.ls, gls'.ls);
+    if (&& gls.ls.environment.nextStep.LEnvStepHostIos? 
+        && gls.ls.environment.nextStep.actor in gls.ls.servers) {
+        // If gls->gls' is a node Grant or Accept step
+        var id, ios := gls.ls.environment.nextStep.actor, gls.ls.environment.nextStep.ios;
+        assert id in config;
+        assert NodeNext(gls.ls.servers[id], gls'.ls.servers[id], ios);
+
+        if NodeGrant(gls.ls.servers[id], gls'.ls.servers[id], ios) {
+            if gls.ls.servers[id].held && gls.ls.servers[id].epoch < 0xFFFF_FFFF_FFFF_FFFF {
+                assert false;  // contradics NoLockHolder(config, gls);
+            } else {
+                assert gls'.ls.servers == gls.ls.servers;
+                assert gls'.ls.environment.sentPackets == gls.ls.environment.sentPackets;
+            }
+        } else {
+            assert NodeAccept(gls.ls.servers[id], gls'.ls.servers[id], ios);
+            if ios[0].LIoOpTimeoutReceive? {
+                assert gls'.ls.servers == gls.ls.servers;
+                assert gls'.ls.environment.sentPackets == gls.ls.environment.sentPackets;
+            } else {
+                if (!gls.ls.servers[id].held 
+                    && ios[0].r.src in gls.ls.servers[id].config
+                    && ios[0].r.msg.Transfer? 
+                    && ios[0].r.msg.transfer_epoch > gls.ls.servers[id].epoch)
+                {
+                    assert gls'.ls.servers[id].held;
+                    assert !NoLockHolder(config, tgls');
+                    assert forall id' | id' in config && id' != id :: !gls.ls.servers[id'].held;
+                    forall p | p in gls'.ls.environment.sentPackets  
+                    ensures !IsInFlightTransferMessage(config, tgls', p)
+                    {
+                        if p.dst in config && p.src in config && p.msg.Transfer? {
+                            assert p in gls.ls.environment.sentPackets;
+                            if p.dst == id {
+                                if p.msg.transfer_epoch > gls.ls.servers[id].epoch {
+                                    var receivedMessage := ios[0].r;
+                                    assert IsValidLIoOp(ios[0], id, gls.ls.environment);
+                                    assert receivedMessage.dst == id;
+                                    assert IsInFlightTransferMessage(config, tgls, receivedMessage);
+                                    assert IsInFlightTransferMessage(config, tgls, p);
+                                    assert p == receivedMessage;
+                                    assert p.msg.transfer_epoch == gls'.ls.servers[id].epoch;
+                                    assert !IsInFlightTransferMessage(config, tgls', p);
+                                } else {
+                                    assert !IsInFlightTransferMessage(config, tgls', p);
+                                }
+                            } else {
+                                assert gls'.ls.servers[p.dst].epoch == gls.ls.servers[p.dst].epoch;
+                                assert gls.ls.servers[p.dst].epoch >= p.msg.transfer_epoch;
+                            }
+                        }
+                    }
+                    assert HistoryLengthInvariant(config, tgls');  // Dafny magic!
+                } else {
+                    assert gls'.ls.servers == gls.ls.servers;
+                    assert gls'.ls.environment.sentPackets == gls.ls.environment.sentPackets;
+                }
+            }
+        }
+        assert HistoryLengthInvariant(config, tgls');
+    } else {
+        // If gls->gls' is purely an environment step
+        // (not gls.ls.environment.nextStep.LEnvStepHostIos?) or (not gls.ls.environment.nextStep.actor in gls.ls.servers)
+        assert gls.ls.servers == gls'.ls.servers && gls.history == gls'.history;
+        if !gls.ls.environment.nextStep.LEnvStepHostIos? {
+            match gls.ls.environment.nextStep {
+                case LEnvStepHostIos(actor, ios, nodestep) => assert false;
+                case LEnvStepDeliverPacket(p) => assert LEnvironment_Stutter(gls.ls.environment, gls'.ls.environment);
+                case LEnvStepAdvanceTime => assert LEnvironment_AdvanceTime(gls.ls.environment, gls'.ls.environment);
+                case LEnvStepStutter => assert LEnvironment_Stutter(gls.ls.environment, gls'.ls.environment);
+            }
+            assert gls'.ls.environment.sentPackets == gls.ls.environment.sentPackets;
+        } else {
+            assert gls.ls.environment.nextStep.actor !in gls.ls.servers;
+            if gls.ls.environment.nextStep.LEnvStepHostIos? {  
+                // Any message sent in this step cannot be classified as InFlight 
+                // because their source == actor is not in config
+                assert OneTransferMessageIsInFlight(config, tgls);
+                var id, ios := gls.ls.environment.nextStep.actor, gls.ls.environment.nextStep.ios;
+                forall io | io in ios && io.LIoOpSend?
+                ensures !IsInFlightTransferMessage(config, tgls', io.s)
+                {}
+                assert gls'.ls.environment.sentPackets == gls.ls.environment.sentPackets + (set io | io in ios && io.LIoOpSend? :: io.s);
+                assert forall p | p in gls'.ls.environment.sentPackets && IsInFlightTransferMessage(config, tgls', p) :: p in gls.ls.environment.sentPackets;
+                assert NoLockHolder(config, tgls');
+                assert OneTransferMessageIsInFlight(config, tgls');
+            } else {
+                assert gls'.ls.environment.sentPackets == gls.ls.environment.sentPackets;
+            }
+        }
+        assert HistoryLengthInvariant(config, tgls');
+    }
+}
+}
