ironfleet/src/Dafny/Distributed/Protocol/Lock/PerformanceProofNQ/DefinitionsNQ.i.dfy
@@ -1,0 +1,76 @@
+// Must be verified with /arith:2
+
+include "../../../Services/Lock/LockTimestampedDistributedSystem.i.dfy"
+
+module PerformanceProof__Definitions_i {
+import opened LockTimestampedDistributedSystem_i
+
+ghost const Gs := StepTime(GrantStep);
+ghost const As := StepTime(AcceptStep);
+ghost const Ds := DeliveryTime();
+ghost const G:Timestamp
+ghost const A:Timestamp
+ghost const D:Timestamp
+
+function StepToTimeDelta(hstep:HostStep) : Timestamp
+{
+  if hstep == GrantStep then G else A
+}
+
+function TLS_NoRecvPerfUpdate(node_pr:Timestamp, hstep:HostStep) : Timestamp
+{
+  var total_time := TimeAdd2(node_pr, StepToTimeDelta(hstep));
+  total_time
+}
+
+function TLS_RecvPerfUpdate(node_pr:Timestamp, pkt_pr:Timestamp, hstep:HostStep) : Timestamp
+{
+  var deliveryTime := TimeAdd2(pkt_pr, D);  // add D to packet sent time
+  // var handlerStartTime := TimeMax(deliveryTime, node_pr);   
+  var total_time := TimeAdd2(deliveryTime, StepToTimeDelta(hstep));
+  total_time
+}
+
+function PerfBoundLockHeld(epoch: int) : Timestamp
+  requires 0 < epoch
+  ensures PerfBoundLockHeld(epoch) >= 0
+{
+  (epoch - 1) * G + (epoch - 1) * A + (epoch - 1) * D
+}
+
+function PerfBoundLockInNetwork(epoch: int) : Timestamp
+  requires 0 < epoch
+  ensures PerfBoundLockInNetwork(epoch) >= 0
+{
+  if epoch == 1 then  // note that a valid Transfer packet never has epoch 0
+    0
+  else
+    (epoch - 1) * G + (epoch - 2) * A + (epoch - 2) * D
+}
+
+predicate TimeEq(p1:Timestamp, p2:Timestamp)
+{
+  p1 == p2
+}
+
+predicate TimeLe(p1:Timestamp, p2:Timestamp)
+{
+  p1 <= p2
+}
+
+lemma Grant_j_helper_specific(epoch:int)
+  requires epoch > 0
+  ensures TimeEq(PerfBoundLockInNetwork(epoch + 1), TimeAdd2(PerfBoundLockHeld(epoch), G));
+{
+}
+
+lemma Grant_j_helper()
+  ensures forall epoch :: epoch > 0 ==> TimeEq(PerfBoundLockInNetwork(epoch + 1), TimeAdd2(PerfBoundLockHeld(epoch), G));
+{
+}
+
+lemma Accept_j_helper()
+  ensures forall epoch :: epoch > 1 ==> TimeEq(PerfBoundLockHeld(epoch), TLS_RecvPerfUpdate(TimeVoid(), PerfBoundLockInNetwork(epoch), AcceptStep))
+{
+}
+}
