ironfleet/src/Dafny/Distributed/Protocol/Lock/PerformanceProofNQ/MultiRoundPerformanceProof.i.dfy
@@ -1,0 +1,269 @@
+include "../../../Services/Lock/LockTimestampedDistributedSystem.i.dfy"
+include "TimestampedGLS_noduplication.i.dfy"
+include "DefinitionsNQ.i.dfy"
+include "../../../../Libraries/Math/mod_auto.i.dfy"
+include "MultiRoundTimeHelpers.i.dfy"
+include "../../../Common/Collections/Multisets.s.dfy"
+
+module MultiRoundPerformanceProof_i {
+
+import opened LockTimestampedDistributedSystem_i
+  import opened TimestampedGLS_noduplication_i
+  import opened PerformanceProof__Definitions_i
+  import opened Math__mod_auto_i
+  import opened PerformanceProof__MultiRoundTimeHelpers_i
+  import opened Collections__Multisets_s
+
+predicate NoPacketDuplication(tls:TimestampedLS_State)
+{
+  var nextStep := tls.t_environment.nextStep;
+  nextStep.LEnvStepHostIos? ==> (
+  (forall io :: io in nextStep.ios && io.LIoOpReceive? ==> io.r in tls.undeliveredPackets)
+  )
+}
+
+predicate LockedPacketNeverDelivered(tls:TimestampedLS_State)
+{
+  var nextStep := tls.t_environment.nextStep;
+  nextStep.LEnvStepHostIos? ==> (forall io :: io in nextStep.ios && io.LIoOpReceive? ==> !io.r.msg.v.Locked?)
+}
+
+predicate SingleGLSPerformanceAssumption(tgls:TimestampedGLS_State)
+{
+  && NoPacketDuplication(tgls.tls)
+  && LockedPacketNeverDelivered(tgls.tls)
+
+  // The only nodes that take steps are in the ring
+  && (tgls.tls.t_environment.nextStep.LEnvStepHostIos? ==> tgls.tls.t_environment.nextStep.actor in tgls.tls.t_servers)
+
+  // The size of the history/epochs never reaches UINT64_MAX
+  && (|tgls.history| < 0xFFFF_FFFF_FFFF_FFFF)
+
+  // No timeouts
+  && (var nextStep := tgls.tls.t_environment.nextStep; nextStep.LEnvStepHostIos? ==>
+  (forall io :: io in nextStep.ios ==> !io.LIoOpTimeoutReceive?))
+  
+  // No 'Locked' packets are ever received
+  && (var nextStep := tgls.tls.t_environment.nextStep; nextStep.LEnvStepHostIos? ==>
+  (forall io :: io in nextStep.ios && io.LIoOpReceive? ==> io.r.msg.v.Locked? == false))
+
+  // TODO: This should be part of the state machine definition, and not an assumption
+  // The only nodes that can do NodeGrant() currently hold the lock
+  && (var nextStep := tgls.tls.t_environment.nextStep; nextStep.LEnvStepHostIos? ==> (nextStep.nodeStep == GrantStep <==> tgls.tls.t_servers[nextStep.actor].v.held == true))
+
+}
+
+predicate GLSPerformanceAssumption(tglb:seq<TimestampedGLS_State>)
+{
+  forall tgls :: tgls in tglb ==> SingleGLSPerformanceAssumption(tgls)
+}
+
+predicate SingleGLSPerformanceGuarantee(gls:TimestampedGLS_State)
+{
+  |gls.tls.config| > 1 ==> 
+  (forall pkt :: pkt in gls.tls.t_environment.sentPackets &&
+    pkt.msg.v.Transfer? ==> pkt.msg.v.transfer_epoch > 1 && TimeLe(pkt.msg.ts, PerfBoundLockInNetwork(pkt.msg.v.transfer_epoch)))
+}
+
+predicate GLSPerformanceGuarantee(tglb:seq<TimestampedGLS_State>)
+{
+  forall tgls :: tgls in tglb ==> SingleGLSPerformanceGuarantee(tgls)
+}
+
+predicate TGLS_Consistency(tgls: TimestampedGLS_State)
+{
+  && (forall id :: id in tgls.tls.config <==> id in tgls.tls.t_servers)
+    && (forall id :: id in tgls.tls.t_servers ==> (tgls.tls.t_servers[id].v.config == tgls.tls.config))
+    && (forall i :: 0 <= i < |tgls.tls.config| ==> tgls.tls.t_servers[tgls.tls.config[i]].v.my_index == i)
+}
+
+predicate NoTransferPackets(pkts:multiset<TimestampedLPacket<EndPoint, LockMessage>>)
+{
+  (forall pkt :: pkt in pkts && pkt.msg.v.Transfer? ==> false)
+}
+
+predicate PerfInvariant_LockHeld(tgls:TimestampedGLS_State)
+{
+  |tgls.history| > 0
+  && (forall h :: h in tgls.history ==> h in tgls.tls.t_servers)
+  && tgls.tls.t_servers[tgls.history[|tgls.history| - 1]].v.held
+  && tgls.tls.t_servers[tgls.history[|tgls.history| - 1]].v.epoch == |tgls.history|
+
+  && (forall id :: id in tgls.tls.t_servers && id != tgls.history[|tgls.history| - 1]
+  ==> !tgls.tls.t_servers[id].v.held
+          && tgls.tls.t_servers[id].v.epoch < |tgls.history|
+  )
+  && NoTransferPackets(tgls.tls.undeliveredPackets)
+}
+
+
+predicate PerfInvariant_LockNotHeld(tgls:TimestampedGLS_State)
+{
+  |tgls.history| > 0
+  && (forall id :: id in tgls.tls.t_servers
+      ==> !tgls.tls.t_servers[id].v.held
+          && tgls.tls.t_servers[id].v.epoch < |tgls.history|
+  )
+
+  && (forall pkt :: pkt in tgls.tls.undeliveredPackets && pkt.msg.v.Transfer?
+      ==> pkt.dst == tgls.history[|tgls.history| - 1]
+      && pkt.src in tgls.tls.t_servers
+      && pkt.msg.v.transfer_epoch == |tgls.history|
+      && (var undeliveredPackets' := tgls.tls.undeliveredPackets - multiset({pkt});
+          NoTransferPackets(undeliveredPackets')
+        )
+  )
+}
+
+predicate PerfInvariantAlways_Alt(tgls:TimestampedGLS_State)
+{
+  |tgls.history| > 0
+  && (forall h :: h in tgls.history ==> h in tgls.tls.t_servers)
+
+  // No Invalid packets are ever sent
+  && (forall pkt :: pkt in tgls.tls.undeliveredPackets
+  ==>
+  !pkt.msg.v.Invalid?)
+
+  && (forall id :: id in tgls.tls.t_servers ==> var t_hs := tgls.tls.t_servers[id];
+      && (t_hs.v.held == false ==> 0 <= t_hs.v.epoch < |tgls.history| && TimeLe(t_hs.ts, PerfBoundLockInNetwork(t_hs.v.epoch + 1)))
+      && (t_hs.v.held == true  ==> 0 < t_hs.v.epoch == |tgls.history| && TimeLe(t_hs.ts, PerfBoundLockHeld(t_hs.v.epoch)))
+  )
+
+  && (forall pkt :: pkt in tgls.tls.undeliveredPackets && pkt.msg.v.Transfer?
+  ==> 1 < pkt.msg.v.transfer_epoch && TimeLe(pkt.msg.ts, PerfBoundLockInNetwork(pkt.msg.v.transfer_epoch))
+  )
+
+  && SingleGLSPerformanceGuarantee(tgls)
+
+  && (if tgls.tls.t_servers[tgls.history[|tgls.history| - 1]].v.held then
+    PerfInvariant_LockHeld(tgls)
+  else
+    PerfInvariant_LockNotHeld(tgls)
+    )
+}
+
+lemma NotHostIos_InvariantMaintained(s:TimestampedGLS_State, s':TimestampedGLS_State)
+  requires TGLS_Next(s, s')
+  requires TGLS_Consistency(s) && TGLS_Consistency(s')
+  requires SingleGLSPerformanceAssumption(s)
+
+  requires !s.tls.t_environment.nextStep.LEnvStepHostIos?
+
+  requires PerfInvariantAlways_Alt(s);
+  ensures PerfInvariantAlways_Alt(s');
+{
+}
+
+lemma Grant_InvariantMaintained(s:TimestampedGLS_State, s':TimestampedGLS_State)
+  requires TGLS_Next(s, s')
+  requires TGLS_Consistency(s) && TGLS_Consistency(s')
+  requires SingleGLSPerformanceAssumption(s)
+
+  requires s.tls.t_environment.nextStep.LEnvStepHostIos?
+  requires s.tls.t_environment.nextStep.nodeStep == GrantStep
+
+  requires PerfInvariantAlways_Alt(s);
+  ensures PerfInvariantAlways_Alt(s');
+{
+  var t_hs := s.tls.t_servers[s.tls.t_environment.nextStep.actor];
+  lemma_Grant(t_hs.ts, t_hs.v.epoch);
+}
+
+
+lemma Accept_InvariantMaintained(s:TimestampedGLS_State, s':TimestampedGLS_State)
+  requires TGLS_Next(s, s')
+  requires TGLS_Consistency(s) && TGLS_Consistency(s')
+  requires SingleGLSPerformanceAssumption(s)
+
+  requires s.tls.t_environment.nextStep.LEnvStepHostIos?
+  requires s.tls.t_environment.nextStep.nodeStep == AcceptStep
+
+  requires PerfInvariantAlways_Alt(s);
+  ensures PerfInvariantAlways_Alt(s');
+{
+  var id := s.tls.t_environment.nextStep.actor;
+  var t_hs := s.tls.t_servers[id];
+  var ios := s.tls.t_environment.nextStep.ios;
+  assert IsValidLIoOp(ios[0], id, s.tls.t_environment);
+  var pkt := ios[0].r;
+  assert pkt.msg.v.Transfer?;
+
+  // These two lines are not necessary, but they seem to speed up verification of this lemma
+  var s_pkt := ios[1].s;
+  assert !s_pkt.msg.v.Transfer?;
+
+  lemma_Accept(s.tls.t_servers[id].ts, pkt.msg.ts, s.tls.t_servers[id].v.epoch, pkt.msg.v.transfer_epoch);
+}
+
+lemma InitImpliesInvariant(s:TimestampedGLS_State)
+  requires TGLS_Init(s, s.tls.config)
+  requires TGLS_Consistency(s)
+  ensures PerfInvariantAlways_Alt(s)
+{
+}
+
+lemma TGLS_Next_InvariantMaintained(s:TimestampedGLS_State, s':TimestampedGLS_State)
+  requires TGLS_Next(s, s')
+  requires TGLS_Consistency(s) && TGLS_Consistency(s')
+  requires SingleGLSPerformanceAssumption(s)
+  requires PerfInvariantAlways_Alt(s);
+
+  ensures PerfInvariantAlways_Alt(s');
+{
+  if s.tls.t_environment.nextStep.LEnvStepHostIos? {
+    if s.tls.t_environment.nextStep.nodeStep == GrantStep {
+      Grant_InvariantMaintained(s, s');
+    }
+    else {
+      Accept_InvariantMaintained(s, s');
+    }
+  }
+  else {
+   NotHostIos_InvariantMaintained(s, s'); 
+  }
+}
+
+lemma InvariantImpliesGuarantee(s:TimestampedGLS_State)
+  requires PerfInvariantAlways_Alt(s);
+  ensures SingleGLSPerformanceGuarantee(s)
+{
+  
+}
+
+lemma Establish_TGLS_Consistency(config:Config, tglb:seq<TimestampedGLS_State>, i:int)
+  requires ValidTimestampedGLSBehavior(tglb, config)
+  requires 0 <= i < |tglb|
+  ensures TGLS_Consistency(tglb[i])
+
+  decreases i
+{
+  if i > 0{
+    Establish_TGLS_Consistency(config, tglb, i - 1);
+  }
+}
+
+
+lemma PerformanceGuaranteeHolds(config:Config, tglb:seq<TimestampedGLS_State>)
+  requires ValidTimestampedGLSBehavior(tglb, config)
+  requires GLSPerformanceAssumption(tglb)
+  ensures GLSPerformanceGuarantee(tglb)
+{
+  var i := 0;
+  Establish_TGLS_Consistency(config, tglb, 0);
+  InitImpliesInvariant(tglb[0]);
+
+  while i < |tglb| - 1
+    invariant 0 <= i < |tglb|
+    invariant GLSPerformanceGuarantee(tglb[..i+1])
+    invariant PerfInvariantAlways_Alt(tglb[i])
+  {
+    Establish_TGLS_Consistency(config, tglb, i);
+    Establish_TGLS_Consistency(config, tglb, i + 1);
+    TGLS_Next_InvariantMaintained(tglb[i], tglb[i + 1]);
+    InvariantImpliesGuarantee(tglb[i+1]);
+    i := i + 1;
+  }
+}
+
+}
