ironfleet/src/Dafny/Distributed/Protocol/Lock/PerformanceProofNQ/TimestampedGLS_noduplication.i.dfy
@@ -1,0 +1,122 @@
+include "../../Lock/Node.i.dfy"
+include "../RefinementProof/DistributedSystem.i.dfy"
+include "../../../Services/Lock/LockTimestampedDistributedSystem.i.dfy"
+include "DefinitionsNQ.i.dfy"
+
+module TimestampedGLS_noduplication_i {
+import opened Protocol_Node_i
+import opened DistributedSystem_i
+import opened LockTimestampedDistributedSystem_i
+import opened PerformanceProof__Definitions_i
+
+type TimestampedNode = TimestampedType<Node>
+  
+datatype TimestampedLS_State = TimestampedLS_State(
+  config:ConcreteConfiguration,
+  t_environment:TimestampedLEnvironment<EndPoint, LockMessage, HostStep>,
+  t_servers:map<EndPoint,TimestampedNode>,
+  undeliveredPackets:multiset<TimestampedLPacket<EndPoint, LockMessage>>
+  )
+
+datatype TimestampedGLS_State = TimestampedGLS_State(
+  tls:TimestampedLS_State,
+  history:seq<EndPoint>
+  )
+
+  function UntagLSServers(t_servers: map<EndPoint, TimestampedNode>) : map<EndPoint, Node>
+  {
+    map id | id in t_servers :: t_servers[id].v
+  }
+
+  function UntagLS_State(tds:TimestampedLS_State) : LS_State
+  {
+    LS_State(
+      UntagLEnvironment(tds.t_environment),
+      UntagLSServers(tds.t_servers))
+  }
+
+  predicate TLS_Init(tls: TimestampedLS_State, config:Config)
+    reads *
+  {
+    && LS_Init(UntagLS_State(tls), config)
+      && tls.undeliveredPackets == multiset{}
+      && tls.config == config
+      && LEnvironment_Init(tls.t_environment)
+      && config[0] in tls.t_servers
+      && tls.t_servers[config[0]].ts == TimeZero()
+      && forall id :: id in tls.t_servers && id != config[0] ==> tls.t_servers[id].ts == TimeZero()
+  }
+
+  predicate TLS_NextOneServer(tls: TimestampedLS_State, tls': TimestampedLS_State, id:EndPoint, ios:seq<TimestampedLIoOp<EndPoint, LockMessage>>, hstep:HostStep)
+    requires id in tls.t_servers;
+    reads *
+  {
+    LS_NextOneServer(UntagLS_State(tls), UntagLS_State(tls'), id, UntagLIoOpSeq(ios), hstep)
+      && (if |ios| > 0 && ios[0].LIoOpReceive? then
+        tls'.t_servers[id].ts == TLS_RecvPerfUpdate(tls.t_servers[id].ts, ios[0].r.msg.ts, hstep)
+      else
+        tls'.t_servers[id].ts == TLS_NoRecvPerfUpdate(tls.t_servers[id].ts, hstep)
+        )
+
+      && (forall t_io :: t_io in ios && t_io.LIoOpSend? ==> t_io.s.msg.ts == tls'.t_servers[id].ts)
+      && tls'.t_servers == tls.t_servers[id := tls'.t_servers[id]]
+  }
+
+
+  predicate UndeliveredPackets_Next(tls:TimestampedLS_State, tls':TimestampedLS_State)
+    requires tls.t_environment.nextStep.LEnvStepHostIos?
+  {
+    var nextStep := tls.t_environment.nextStep;
+    var ios := nextStep.ios;
+    tls'.undeliveredPackets == tls.undeliveredPackets -
+      multiset((set io | io in ios && io.LIoOpReceive? :: io.r)) +
+      multiset((set io | io in ios && io.LIoOpSend? :: io.s))
+  }
+
+  predicate TLS_Next(tls:TimestampedLS_State, tls': TimestampedLS_State)
+    reads *
+  {
+    tls.config == tls'.config
+    && LS_Next(UntagLS_State(tls), UntagLS_State(tls'))
+    && LEnvironment_Next(tls.t_environment, tls'.t_environment)
+    && if tls.t_environment.nextStep.LEnvStepHostIos? && tls.t_environment.nextStep.actor in tls.t_servers then
+           TLS_NextOneServer(tls, tls', tls.t_environment.nextStep.actor, tls.t_environment.nextStep.ios, tls.t_environment.nextStep.nodeStep)
+           && UndeliveredPackets_Next(tls, tls')
+       else
+        tls'.t_servers == tls.t_servers
+        && tls'.undeliveredPackets == tls.undeliveredPackets
+
+        && (if tls.t_environment.nextStep.LEnvStepHostIos? then
+            && (forall t_io :: t_io in tls.t_environment.nextStep.ios && t_io.LIoOpSend? ==> t_io.s.msg.ts == TimeZero())
+            else
+            true)
+  }
+
+  predicate TGLS_Init(tgls:TimestampedGLS_State, config:Config)
+    reads *
+  {
+    TLS_Init(tgls.tls, config)
+      && tgls.history == [config[0]]
+  }
+
+  predicate TGLS_Next(tgls:TimestampedGLS_State, tgls':TimestampedGLS_State)
+    reads *
+  {
+    TLS_Next(tgls.tls, tgls'.tls)
+      && (if tgls.tls.t_environment.nextStep.LEnvStepHostIos? && tgls.tls.t_environment.nextStep.actor in tgls.tls.t_servers
+      && NodeGrant(tgls.tls.t_servers[tgls.tls.t_environment.nextStep.actor].v, tgls'.tls.t_servers[tgls.tls.t_environment.nextStep.actor].v, UntagLIoOpSeq(tgls.tls.t_environment.nextStep.ios))
+      && tgls.tls.t_servers[tgls.tls.t_environment.nextStep.actor].v.held && tgls.tls.t_servers[tgls.tls.t_environment.nextStep.actor].v.epoch < 0xFFFF_FFFF_FFFF_FFFF then
+      tgls'.history == tgls.history + [tgls.tls.t_servers[tgls.tls.t_environment.nextStep.actor].v.config[(tgls.tls.t_servers[tgls.tls.t_environment.nextStep.actor].v.my_index + 1) % |tgls.tls.t_servers[tgls.tls.t_environment.nextStep.actor].v.config|]]
+      else
+        tgls'.history == tgls.history
+        )
+  }
+
+  predicate ValidTimestampedGLSBehavior(tglb:seq<TimestampedGLS_State>, config:Config)
+    reads *
+  {
+    && |tglb| > 0
+      && TGLS_Init(tglb[0], config)
+      && (forall i :: 0 < i < |tglb| ==> TGLS_Next(tglb[i - 1], tglb[i]))
+  }
+}
