ironfleet/src/Dafny/Distributed/Protocol/ZooKeeper/DistributedSystem.dfy
@@ -1,0 +1,71 @@
+include "../../Impl/Common/SeqIsUniqueDef.i.dfy"
+include "../../Common/Framework/EnvironmentTCP.s.dfy"
+
+include "Types.dfy"
+include "ZKEnvironment.dfy"
+include "ZKDatabase.dfy"
+include "Follower.dfy"
+include "Leader.dfy"
+include "LearnerHandler_Bug.dfy"
+
+
+module ZooKeeper_DistributedSystem {
+import opened Common__SeqIsUniqueDef_i
+
+import opened ZooKeeper_Types
+import opened ZooKeeper_Environment
+import opened EnvironmentTCP_s
+import opened ZooKeeper_ZKDatabase
+import opened ZooKeeper_Follower
+import opened ZooKeeper_Leader
+import opened ZooKeeper_LearnerHandler
+
+datatype QuorumPeer = LeaderPeer(leader:Leader) | FollowerPeer(follower:Follower)
+
+datatype LS_State = LS_State(
+    environment: ZKEnvironment,
+    initialZkdbState: seq<ZKDatabase>,
+    servers: map<EndPoint, QuorumPeer>
+)
+
+
+predicate LS_Init(config:Config, s:LS_State, f: int) {
+    && f >= 1
+    && LEnvironment_Init(config, s.environment)
+    && |config| == |s.initialZkdbState| == 2*f + 1 // we will assign each server in config the corresponding db
+    && SeqIsUnique(config)
+    && InitialZkdbState_EmptyDiff(s.initialZkdbState)
+    && (forall e :: e in config <==> e in s.servers)
+        // this is the leader
+    && s.servers[config[0]].LeaderPeer?
+    && LeaderInit(s.servers[config[0]].leader, 0, config, s.initialZkdbState[0])
+        // remaining nodes are followers
+    && (forall i | 1 <= i < |config| :: 
+            && s.servers[config[i]].FollowerPeer?
+            && FollowerInit(s.servers[config[i]].follower, i, 0, config, s.initialZkdbState[i])
+    )
+}
+
+
+predicate LS_NextOneServer(s:LS_State, s':LS_State, actor:EndPoint, ios:seq<ZKIo>)
+    requires actor in s.servers
+{
+    && s.environment.nextStep == LEnvStepHostIos(actor, ios)
+    && actor in s'.servers
+    && s'.servers == s.servers[actor := s'.servers[actor]]
+    && match s.servers[actor] 
+        case LeaderPeer(leader) => 
+            && s'.servers[actor].LeaderPeer?
+            && LeaderNext(leader, s'.servers[actor].leader, ios)
+        case FollowerPeer(follower) => 
+            && s'.servers[actor].FollowerPeer?
+            && FollowerNext(follower, s'.servers[actor].follower, ios)
+}
+
+
+predicate LS_Next(s:LS_State, s':LS_State){
+    && LEnvironment_Next(s.environment, s'.environment)
+    && (exists ep, ios :: ep in s.servers && LS_NextOneServer(s, s', ep, ios))
+    && s'.initialZkdbState == s.initialZkdbState
+}
+}
