ironfleet/src/Dafny/Distributed/Protocol/ZooKeeper/LearnerHandler_Bug.dfy
@@ -1,0 +1,274 @@
+include "Types.dfy"
+include "ZKDatabase.dfy"
+include "ZKEnvironment.dfy"
+
+
+module ZooKeeper_LearnerHandler {
+import opened ZooKeeper_Types
+import opened ZooKeeper_ZKDatabase
+import opened ZooKeeper_Environment
+
+
+datatype LearnerHandlerState = 
+                | LH_HANDSHAKE_A | LH_HANDSHAKE_B 
+                | LH_PREP_SYNC | LH_SYNC
+                | LH_PROCESS_ACK
+                | LH_RUNNING | LH_ERROR
+
+datatype SyncMode = SNAP | DIFF | TRUNC
+
+
+datatype LearnerHandler = LearnerHandler(
+    my_id: nat,
+    follower_id: nat,
+    state: LearnerHandlerState,
+
+    // Local state
+    queuedPackets: seq<ZKMessage>,
+    newEpoch: int,
+    peerLastZxid: Zxid
+)
+
+
+/* Global Leader variables shared by all LearnerHandler threads */
+datatype LeaderGlobals = LeaderGlobals(
+    zkdb: ZKDatabase,
+    config: Config,
+
+    // Synchronization globals
+    leaderEpoch: int,
+    currZxid: Zxid,
+    connectingFollowers: set<nat>,
+    nextSerialLI: nat,          // next serial number for LeaderInfo
+    electingFollowers: set<nat>,
+    procEpCount: nat,           // how many times WaitForEpochAck has been run after electingFollowers is declared quorum
+    nextSerialSync: nat,        // next serial number for SyncDIFF | SyncSNAP | SyncTRUNC
+    nextSerialNL: nat,          // next serial number for newLeader
+    prepCount: nat,             // how many times PrepSync has been run
+    ackSet: set<nat>
+)
+
+
+/*****************************************************************************************
+*                                      Actions                                           *
+******************************************************************************************/ 
+
+predicate LearnerHandlerInit(s:LearnerHandler, my_id:nat, follower_id:nat) {
+    && s.my_id == my_id
+    && s.follower_id == follower_id
+    && s.state == LH_HANDSHAKE_A
+
+    && s.queuedPackets == []
+    && s.newEpoch == -1
+    && s.peerLastZxid == NullZxid
+}
+
+predicate LearnerHandlerNext(s:LearnerHandler, s':LearnerHandler, g:LeaderGlobals, g':LeaderGlobals, ios:seq<ZKIo>) {
+    match s.state 
+        case LH_HANDSHAKE_A => GetEpochToPropose(s, s', g, g', ios)
+        case LH_HANDSHAKE_B => WaitForEpochAck(s, s', g, g', ios)
+        case LH_PREP_SYNC => PrepareSync(s, s', g, g', ios)
+        case LH_SYNC => DoSync(s, s', g, g', ios)
+        case LH_PROCESS_ACK => ProcessAck(s, s', g, g', ios)
+        case LH_RUNNING => LearnerHandlerStutter(s, s', ios) && g' == g
+        case LH_ERROR => LearnerHandlerStutter(s, s', ios) && g' == g
+}
+
+predicate LearnerHandlerStutter(s:LearnerHandler, s':LearnerHandler, ios:seq<ZKIo>) {
+    && |ios| == 0
+    && s' == s
+}
+
+/* Process_FI */
+predicate GetEpochToPropose(s:LearnerHandler, s':LearnerHandler, g:LeaderGlobals, g':LeaderGlobals, ios:seq<ZKIo>) 
+    requires s.state == LH_HANDSHAKE_A
+{
+    if IsVerifiedQuorum(s.follower_id, |g.config|, g.connectingFollowers) 
+    then ( // Send Leader.LEADERINFO message to follower, and proceed to LH_HANDSHAKE_B state
+        && g' == g.(nextSerialLI := g.nextSerialLI + 1)
+        && |ios| == 1
+        && s' == s.(state := LH_HANDSHAKE_B, newEpoch := g.leaderEpoch)
+        && ios[0].LIoOpSend?
+        && (var outbound_packet := ios[0].s;
+            && 0 <= s.follower_id < |g.config|
+            && outbound_packet.dst == g.config[s.follower_id]
+            && outbound_packet.sender_index == s.my_id
+            && outbound_packet.msg == LeaderInfo(s.my_id, g.nextSerialLI, Zxid(g.leaderEpoch, 0))
+        )       
+    ) else ( // Add sender to my connectingFollowers set, and continue waiting for quorum
+        // if |ios| == 0 then LearnerHandlerStutter(s, s', ios) && g' == g  // Case where follower has not sent anything
+        // else 
+            && s.follower_id !in g.connectingFollowers
+            && !IsQuorum(|g.config|, g.connectingFollowers)   // Stop accepting new followers after I have a quorum
+            && s.follower_id !in g.connectingFollowers
+            && |ios| == 1
+            && ios[0].LIoOpReceive?
+            && ios[0].r.src in g.config
+            && ios[0].r.msg.FollowerInfo?
+            && 0 <= ios[0].r.msg.sid < |g.config| 
+            && ios[0].r.msg.sid == s.follower_id
+            && g.config[ios[0].r.msg.sid] == ios[0].r.src
+            && s' == s.(
+                follower_id := ios[0].r.msg.sid,
+                peerLastZxid := ios[0].r.msg.latestZxid
+            ) 
+            && g' == g.(
+                leaderEpoch := (if ios[0].r.msg.latestZxid.epoch >= g.leaderEpoch then ios[0].r.msg.latestZxid.epoch + 1 else g.leaderEpoch),
+                connectingFollowers := g.connectingFollowers + {ios[0].r.msg.sid},
+                currZxid := (if ios[0].r.msg.latestZxid.epoch >= g.leaderEpoch then Zxid(ios[0].r.msg.latestZxid.epoch + 1, 0) else g.currZxid)
+            ) 
+    )
+}
+
+
+predicate WaitForEpochAck(s:LearnerHandler, s':LearnerHandler, g:LeaderGlobals, g':LeaderGlobals, ios:seq<ZKIo>) 
+    requires s.state == LH_HANDSHAKE_B
+{
+    if IsVerifiedQuorum(s.follower_id, |g.config|, g.electingFollowers) 
+    then (
+        // Proceed to state sync
+        g' == g.(procEpCount := g.procEpCount + 1)
+        && |ios| == 0   
+        && s' == s.(state := LH_PREP_SYNC)
+    ) else (
+        // Add sender to my electingFollowers set, store peerLastZxid, and continue waiting for quorum
+        // if |ios| == 0 then LearnerHandlerStutter(s, s', ios) && g' == g // Case where follower has not sent anything
+        // else 
+            && |ios| == 1
+            && !IsQuorum(|g.config|, g.electingFollowers)   // Stop accepting new followers after I have a quorum
+            && s.follower_id !in g.electingFollowers
+            && ios[0].LIoOpReceive?
+            && ios[0].r.src in g.config
+            && ios[0].r.msg.AckEpoch?
+            && 0 <= s.follower_id < |g.config| 
+            && g.config[s.follower_id] == ios[0].r.src
+            && ios[0].r.msg.sid == s.follower_id
+            && s' == s.(peerLastZxid := ios[0].r.msg.lastLoggedZxid)
+            && g' == g.(
+                electingFollowers := g.electingFollowers + {ios[0].r.msg.sid}
+        )
+    )
+}
+
+
+predicate PrepareSync(s:LearnerHandler, s':LearnerHandler, g:LeaderGlobals, g':LeaderGlobals, ios:seq<ZKIo>) 
+    requires s.state == LH_PREP_SYNC
+{
+    if ! (g.zkdb.initialized && isValidZKDatabase(g.zkdb)) then |ios| == 0 && s' == s.(state := LH_ERROR) && g' == g
+    else
+    var proposals := getInMemorySuffix(g.zkdb);
+    && |ios| == 0  // no I/O in this step
+    && s' == s.(state := s'.state)  //syncMode to be modified accordingly
+    && g' == g.(prepCount := g.prepCount + 1)
+    // Initialize all message serial to 0, and only update them to their correct order as I send them out
+    && if |proposals| > 0 
+        then (
+            if ZxidLt(g.zkdb.maxCommittedLog, s.peerLastZxid) 
+            then    && s'.state == LH_SYNC
+                    && s'.queuedPackets == [SyncTRUNC(s.my_id, 0, g.zkdb.maxCommittedLog)]
+            else if ZxidLt(s.peerLastZxid, g.zkdb.minCommittedLog) 
+            then && s'.state == LH_SYNC
+                 && s'.queuedPackets == [SyncSNAP(s.my_id, 0, g.zkdb, getLastLoggedZxid(g.zkdb))]
+            else  // peerLastZxid is in the range of my proposals list
+                if s.peerLastZxid !in proposals then s' == s.(state := LH_ERROR) 
+                else
+                && s'.state == LH_SYNC
+                && s'.queuedPackets == [SyncDIFF(s.my_id, 0, s.peerLastZxid)] + PrepareDiffCommits(s.my_id, proposals, s.peerLastZxid)
+       ) else (
+            if ZxidEq(g.currZxid, s.peerLastZxid)  // THIS IS THE BUG
+            then 
+                // Sync empty diff
+                && s'.state == LH_SYNC
+                && s'.queuedPackets == [SyncDIFF(s.my_id, 0, s.peerLastZxid)]
+            else 
+                // Default to sync entire snapshot. This is the bug.
+                && s'.state == LH_SYNC
+                && s'.queuedPackets == [SyncSNAP(s.my_id, 0, g.zkdb, getLastLoggedZxid(g.zkdb))]
+       )
+}
+
+
+predicate DoSync(s:LearnerHandler, s':LearnerHandler, g:LeaderGlobals, g':LeaderGlobals, ios:seq<ZKIo>) 
+    requires s.state == LH_SYNC
+{
+    && |ios| == 1 
+    && ios[0].LIoOpSend?
+    && 0 <= s.follower_id < |g.config| 
+    && ios[0].s.sender_index == s.my_id
+    && ios[0].s.dst == g.config[s.follower_id]
+    && if |s.queuedPackets| == 0 
+        then // Done with sync. Send NewLeader msg
+            g' == g.(nextSerialNL := g.nextSerialNL + 1)
+            && s' == s.(state := LH_PROCESS_ACK)
+            && ios[0].s.msg == NewLeader(s.my_id, g.nextSerialNL, getLastLoggedZxid(g.zkdb))
+        else // Send next item in queuedPackets. Remain in LH_SYNC state
+            && s' == s.(queuedPackets := s.queuedPackets[1..])
+            && var qp := s.queuedPackets[0];
+            && if qp.SyncDIFF?
+                then && ios[0].s.msg == SyncDIFF(qp.sid, g.nextSerialSync, qp.lastProcessedZxid)
+                     && g' == g.(nextSerialSync := g.nextSerialSync + 1)      
+                else if qp.SyncSNAP?
+                then && ios[0].s.msg == SyncSNAP(qp.sid, g.nextSerialSync, qp.leaderDb, qp.lastProcessedZxid)
+                     && g' == g.(nextSerialSync := g.nextSerialSync + 1)
+                else 
+                    false  // In our environment SNAP and DIFF are the only possibilities      
+}
+
+
+predicate ProcessAck(s:LearnerHandler, s':LearnerHandler, g:LeaderGlobals, g':LeaderGlobals, ios:seq<ZKIo>) 
+    requires s.state == LH_PROCESS_ACK
+{
+    // Leader is in charge of checking AckSet and starting the actual local DB
+    && 0 <= s.follower_id < |g.config| 
+    && if g.zkdb.isRunning  // Leader is in charge of starting db once AckSet is a good quorum
+    then (
+        // Proceed to Running state, send UPTODATE to follower
+        // && s' == s.(state := LH_RUNNING)
+        // && g' == g
+        // && |ios| == 1
+        // && ios[0].LIoOpSend?
+        // && ios[0].s.dst == g.config[s.follower_id]
+        // && ios[0].s.sender_index == s.my_id
+        // && ios[0].s.msg == UpToDate(s.my_id)
+        LearnerHandlerStutter(s, s', ios)
+    ) else (
+        // Add sender to my ackSet set, store peerLastZxid, and continue waiting for quorum
+        // if |ios| == 0 then LearnerHandlerStutter(s, s', ios)  && g' == g // Case where follower has not sent anything
+        // else 
+            && |ios| == 1
+             && ios[0].LIoOpReceive?
+             && s.follower_id !in g.ackSet
+             && ios[0].r.msg.sid == s.follower_id
+             && ios[0].r.src in g.config
+             && ios[0].r.msg.Ack?
+             && g.config[s.follower_id] == ios[0].r.src
+             && s' == s
+             && g' == g.(ackSet := g.ackSet + {ios[0].r.msg.sid})
+    )
+}
+
+
+
+/*****************************************************************************************
+*                                    Helper defs                                         *
+******************************************************************************************/ 
+
+predicate IsVerifiedQuorum(my_id:nat, n:int, quorum: set<nat>) {
+    && my_id in quorum
+    && IsQuorum(n, quorum)
+}
+
+predicate IsQuorum(n:int, quorum: set<nat>) {
+    && |quorum| >= (n/2) + 1
+}
+
+function PrepareDiffCommits(leaderId:nat, proposals:seq<Zxid>, peerLastZxid:Zxid) : seq<ZKMessage> 
+    decreases proposals
+    ensures forall msg | msg in PrepareDiffCommits(leaderId, proposals, peerLastZxid) ::
+        msg.Commit?
+{
+    if |proposals| == 0 then []
+    else if peerLastZxid in proposals then PrepareDiffCommits(leaderId, proposals[1..], peerLastZxid)
+    else [Commit(leaderId, 0, proposals[0])] + PrepareDiffCommits(leaderId, proposals[1..], peerLastZxid)
+}
+}
