ironfleet/src/Dafny/Distributed/Protocol/ZooKeeper/PerformamceProof/Commons.dfy
@@ -1,0 +1,116 @@
+include "../../../Impl/Common/SeqIsUniqueDef.i.dfy"
+include "../../../Common/Framework/EnvironmentTCP.s.dfy"
+include "../Timestamps/TimestampedType.dfy"
+include "TimestampedLS.dfy"
+
+include "../Types.dfy"
+include "../DistributedSystem.dfy"
+include "../ZKEnvironment.dfy"
+include "../ZKDatabase.dfy"
+include "../Follower.dfy"
+include "../Leader.dfy"
+include "../LearnerHandler_Bug.dfy"
+include "Definitions.dfy"
+
+
+/* This module contains some common lemmas */
+module Zookeeper_Commons {
+import opened Common__SeqIsUniqueDef_i
+import opened ZKTimestamp
+import opened ZooKeeper_Types
+import opened ZooKeeper_Environment
+import opened ZooKeeper_DistributedSystem
+import opened EnvironmentTCP_s
+import opened ZooKeeper_ZKDatabase
+import opened ZooKeeper_Follower
+import opened ZooKeeper_Leader
+import opened ZooKeeper_LearnerHandler
+import opened Zookeeper_Performance_Definitions
+import opened ZooKeeper_TimestampedDistributedSystem
+
+
+lemma lemma_Math_Inequality(a:nat, b:nat)
+    requires a <= b + 1
+    ensures b-a+1 >= 0
+{}
+
+lemma lemma_Math_Addition()
+    ensures forall x:Timestamp, a:Timestamp :: x <= x + a
+{}
+
+lemma lemma_Math_Addition_2(x:Timestamp, a:Timestamp)
+    ensures x <= x + a
+{}
+
+
+lemma {:axiom} lemma_Math_Mult_a()
+    ensures forall x | x >= 0 ::
+        forall a, b | a>=0 && b>= a>= 0 :: x*b >= x*a
+{}
+
+lemma lemma_Math_Mult_b()
+    ensures forall x:Timestamp, n:nat ::
+    x * n + x == x * (n+1)
+{}
+
+
+lemma {:axiom} lemma_Math_MaxOfInequalities(a:Timestamp, b:Timestamp, x:Timestamp, y:Timestamp)
+    requires x <= y
+    requires a <= x && b <= y
+    ensures TimeMax(a, b) <= y
+{}
+
+lemma {:axiom} lemma_Math_Inequalities_Mult()
+    ensures forall t:Timestamp, x:nat :: t * x >= 0
+{}
+
+
+lemma {:axiom} lemma_Math_Inequalities_CommonMult(x:Timestamp, a:Timestamp, b:Timestamp)
+    requires a <= b
+    ensures x * a <= x * b
+{}
+
+
+lemma lemma_Size_of_Supeset<T>(s:set<T>) 
+    ensures forall subset:set<T> | s >= subset :: |s| >= |subset|
+{
+    forall subset:set<T> | s >= subset
+    ensures |s| >= |subset|
+    {
+        if |s| < |subset| {
+            assert |s-subset| > 0;
+        }
+    }
+}
+
+lemma lemma_Size_of_Supeset_2<T>(s1:set<T>, s2:set<T>) 
+    requires forall e | e in s1 :: e in s2
+    ensures |s2| >= |s1|;
+{
+    lemma_Size_of_Supeset(s2);
+}
+
+
+lemma lemma_Size_One_Sets<T>(s:set<T>, e:T) 
+    requires s >= {e}
+    requires |s| <= 1
+    ensures s == {e}
+{
+    if s != {e} {
+        if s == {} {
+            assert ! (s >= {e});
+        } else {
+            assert |s| == 1;
+            forall e' | e' in s 
+            ensures e' == e {
+                if e' != e {
+                    assert e' in s && e in s;
+                    assert s >= {e', e};
+                    assert |{e', e}| == 2;
+                    lemma_Size_of_Supeset(s);
+                }
+            }
+        }
+    }
+}
+}
