ironfleet/src/Dafny/Distributed/Protocol/ZooKeeper/PerformamceProof/PerformancePredicates_Bug.dfy
@@ -1,0 +1,422 @@
+include "../../../Impl/Common/SeqIsUniqueDef.i.dfy"
+include "../../../Common/Framework/EnvironmentTCP.s.dfy"
+include "../Timestamps/TimestampedType.dfy"
+include "TimestampedLS.dfy"
+include "ProtocolInvariants.dfy"
+
+include "../Types.dfy"
+include "../DistributedSystem.dfy"
+include "../ZKEnvironment.dfy"
+include "../ZKDatabase.dfy"
+include "../Follower.dfy"
+include "../Leader.dfy"
+include "../LearnerHandler_Bug.dfy"
+include "Definitions.dfy"
+include "Commons.dfy"
+
+
+module Zookeeper_PerformancePredicates {
+import opened Common__SeqIsUniqueDef_i
+import opened ZKTimestamp
+import opened ZooKeeper_Types
+import opened ZooKeeper_Environment
+import opened ZooKeeper_DistributedSystem
+import opened EnvironmentTCP_s
+import opened ZooKeeper_ZKDatabase
+import opened ZooKeeper_Follower
+import opened ZooKeeper_Leader
+import opened ZooKeeper_LearnerHandler
+import opened Zookeeper_Performance_Definitions
+import opened ZooKeeper_TimestampedDistributedSystem
+import opened Zookeeper_ProtocoIInvariants
+import opened Zookeeper_Commons
+
+
+/*****************************************************************************************
+*                                      Assumptions                                       *
+*****************************************************************************************/
+
+
+predicate General_LS_Performance_Assumption(tls:TLS_State) {
+    // The only nodes that take steps are in the ring
+    && (tls.t_environment.nextStep.LEnvStepHostIos? 
+        ==> 
+       tls.t_environment.nextStep.actor in tls.t_servers)
+    // No timeouts.
+    && (tls.t_environment.nextStep.LEnvStepHostIos? 
+        ==>
+        (forall io | io in tls.t_environment.nextStep.ios :: !io.LIoOpTimeoutReceive?))
+}
+
+
+/* Performance assumption Empty Diff */
+predicate Performance_Assumption_EmptyDiff(tlb:seq<TLS_State>) {
+    && |tlb| > 0
+    && (forall i | 0 <= i < |tlb| :: General_LS_Performance_Assumption(tlb[i]))
+    && InitialZkdbState_EmptyDiff(tlb[0].initialZkdbState)
+}
+
+
+/*****************************************************************************************
+*                                     Main Guarantee                                     *
+*****************************************************************************************/
+
+/* Performance guarantee Empty Diff for BUGGY Zookeeper
+* Every leader in the RUNNING state has the specified performance formula. 
+* This formula is:
+    SendFI + D                  # Follower send FI 
+    + ProcFI * f                # Leader receive and process FI
+    + ProcFI * f + D            # Leader gets connectingFollowers quorum and send LI for each follower
+    + ProcLI + D                # Follower process LI and sends AckEpoch
+    + ProcEpAck * f             # Leader receives and processes AckEpoch
+    + ProcEpAck * f             # Leader gets electingFollowers and move to PrepSync state
+    + PreSync * f               # Leader does PrepSync for each folllower
+    + SyncSnap * f              # Leader sends SyncSnap message to each follower. No "D" here because "parallel" with next step
+    + Sync * f + D              # Leader sends NewLeader to each follower
+    + ProcSnap + ProcSync + D   # Follower processes SyncSnap, NewLeader, and sends Ack
+    + ProcAck * f               # Leader receives Ack
+ */
+predicate LS_Performance_Guarantee_EmptyDiff(tls:TLS_State) 
+    requires DS_Config_Invariant(tls.config, tls)
+    requires ZK_Config_Invariant(tls.config, tls)
+    requires Quorums_Size_Invariant(tls)
+{   
+    var f, n := tls.f, |tls.config|;
+    var leaderTQP := tls.t_servers[tls.config[0]];
+    IsQuorum(n, leaderTQP.v.leader.globals.ackSet)
+    ==> 
+    leaderTQP.ts <= Ack_Message_ts_Formula(f, f-1) + ProcAck * f
+}
+
+
+predicate Performance_Guarantee_EmptyDiff(config:Config, tlb:seq<TLS_State>)
+    requires forall i | 0 <= i < |tlb| :: DS_Config_Invariant(config, tlb[i])
+    requires forall i | 0 <= i < |tlb| :: ZK_Config_Invariant(config, tlb[i])
+    requires forall i | 0 <= i < |tlb| :: Quorums_Size_Invariant(tlb[i])
+{
+    forall i | 0 <= i < |tlb| :: LS_Performance_Guarantee_EmptyDiff(tlb[i])
+}
+
+
+/*****************************************************************************************
+*                             Handshake Phase Guarantees                                 *
+*****************************************************************************************/
+
+
+predicate FollowerInit_Invariant(tls:TLS_State){
+    forall ep | ep in tls.t_servers :: (
+        && tls.t_servers[ep].v.FollowerPeer? 
+        && tls.t_servers[ep].v.follower.state == F_HANDSHAKE_A
+        ==> 
+        && tls.t_servers[ep].dts == TimeZero()
+        && tls.t_servers[ep].ts == TimeZero()
+    )
+}
+
+function FollowerInfo_Message_ts_Formula() : Timestamp {
+    SendFI + D
+}
+
+/* Every FollowerInfo packet has ts specified by FollowerInfo_Message_Formula */
+predicate FollowerInfo_Message_ts_Invariant(tls:TLS_State) {
+    forall pkt | pkt in tls.t_environment.sentPackets && pkt.msg.v.FollowerInfo?
+    :: pkt.msg.ts == FollowerInfo_Message_ts_Formula()
+}
+
+
+function ProcessFI_PreQuorum_ts_Formula(l:TQuorumPeer) : Timestamp 
+    requires l.v.LeaderPeer?
+    requires |l.v.leader.globals.connectingFollowers| >= 1
+{
+    var connectingFollowers := l.v.leader.globals.connectingFollowers;
+    FollowerInfo_Message_ts_Formula() + ProcFI * (|connectingFollowers|-1)
+}
+
+function ProcessFI_PreQuorum_dts_Formula() : Timestamp {
+    FollowerInfo_Message_ts_Formula()
+}
+
+
+/* Before the leader has a complete connectingFollowers quorum, its ts and dts are 
+* specified by the respective formulas */
+predicate ProcessFI_PreQuorum_Invariant(tls:TLS_State) 
+    requires DS_Config_Invariant(tls.config, tls)
+    requires ZK_Config_Invariant(tls.config, tls)
+    requires Quorums_Size_Invariant(tls)
+{
+    var n := |tls.config|;
+    var leaderTQP := tls.t_servers[tls.config[0]];
+    !IsQuorum(|tls.config|, leaderTQP.v.leader.globals.connectingFollowers)
+    ==> 
+    && leaderTQP.ts <= ProcessFI_PreQuorum_ts_Formula(leaderTQP)
+    && leaderTQP.dts <= ProcessFI_PreQuorum_dts_Formula()
+}
+
+
+//----------------------------------------------------------------------------------------
+
+/* For all followers after sending FollowerInfo messages */
+predicate Follower_HandshakeB_Invariant(tls:TLS_State){
+    forall ep | 
+        && ep in tls.t_servers 
+        && tls.t_servers[ep].v.FollowerPeer? 
+        && tls.t_servers[ep].v.follower.state == F_HANDSHAKE_B
+    ::  && tls.t_servers[ep].dts == TimeZero()
+        && tls.t_servers[ep].ts == SendFI
+}
+
+/* For all LeaderInfo messages sent BEFORE electingFollowers reaches a quorum */
+function LeaderInfo_Message_PreQuorum_ts_Formula(f:int, serial:nat) : Timestamp 
+    requires f >= 1;
+{
+    SendFI + D 
+    + ProcFI * f // Possibly receive at most f FI's
+    + ProcFI * (serial + 1)  // I am the (serial + 1)-th LI to be sent out
+    + D
+}
+
+
+/* Invariant for followers in F_PRESYNC mode */
+predicate Follower_PreSync_Invariant(tls:TLS_State){
+    forall ep | 
+        && ep in tls.t_servers
+        && tls.t_servers[ep].v.FollowerPeer? 
+        && tls.t_servers[ep].v.follower.state == F_PRESYNC
+        && 0 <= tls.t_servers[ep].v.follower.serialLI < tls.f
+    ::  && tls.t_servers[ep].dts <= LeaderInfo_Message_PreQuorum_ts_Formula(tls.f, tls.t_servers[ep].v.follower.serialLI)
+        && tls.t_servers[ep].ts <= LeaderInfo_Message_PreQuorum_ts_Formula(tls.f, tls.t_servers[ep].v.follower.serialLI) + ProcLI
+}
+
+/* For all AckEpoch messages sent BEFORE electingFollowers reaches a quorum */
+function AckEpoch_Message_PreQuorum_ts_Formula(f:int, serial:nat) : Timestamp 
+    requires f >= 1;
+{
+    LeaderInfo_Message_PreQuorum_ts_Formula(f, serial) + ProcLI + D
+}
+
+
+function ProcessEpAck_PreQuorum_ts_Formula(f:int, n:int, l:TQuorumPeer) : Timestamp 
+    requires l.v.LeaderPeer?
+    requires f >= 1
+    requires |l.v.leader.globals.electingFollowers| >= 1;
+    requires |l.v.leader.globals.connectingFollowers| >= 1;
+    requires !IsQuorum(n, l.v.leader.globals.electingFollowers)
+{
+    var connectingFollowers, electingFollowers := l.v.leader.globals.connectingFollowers, l.v.leader.globals.electingFollowers;
+    if |electingFollowers| <= 1 then 
+        // Have not received any AckEpochs. Dts is from last FollowerInfo received
+        // ts is from receiving |cf| FI's, and sending out #serial of them
+        FollowerInfo_Message_ts_Formula()
+        + ProcFI * (|connectingFollowers|-1)
+        + ProcFI * l.v.leader.globals.nextSerialLI
+    else 
+        AckEpoch_Message_PreQuorum_ts_Formula(f, f-1)
+        + ProcEpAck * (|electingFollowers|-1) // Add processing time
+}
+
+
+function ProcessEpAck_PreQuorum_dts_Formula(f:int, n:int, l:TQuorumPeer) : Timestamp 
+    requires l.v.LeaderPeer?
+    requires f >= 1
+    requires !IsQuorum(n, l.v.leader.globals.electingFollowers)
+{
+    var electingFollowers := l.v.leader.globals.electingFollowers;
+    if |electingFollowers| <= 1 then 
+        // Have not received any AckEpochs. Dts is from last FollowerInfo received
+        FollowerInfo_Message_ts_Formula()
+    else 
+        // From the last AckEpoch I received
+        // The largest AckEpoch serial I can get is f
+        AckEpoch_Message_PreQuorum_ts_Formula(f, f-1)
+}
+
+//----------------------------------------------------------------------------------------
+
+/* Summary of handshake B phase messages */
+predicate Handshake_Messages_Invariant(tls:TLS_State) 
+    requires DS_Config_Invariant(tls.config, tls)
+    requires ZK_Config_Invariant(tls.config, tls)
+{   
+    && (forall pkt | pkt in tls.t_environment.sentPackets && pkt.msg.v.LeaderInfo? // && pkt.msg.v.serial < tls.f
+    :: pkt.msg.ts <= LeaderInfo_Message_PreQuorum_ts_Formula(tls.f, pkt.msg.v.serial))
+    && (forall pkt | pkt in tls.t_environment.sentPackets && pkt.msg.v.AckEpoch?  // && pkt.msg.v.serial < tls.f
+    :: pkt.msg.ts <= AckEpoch_Message_PreQuorum_ts_Formula(tls.f, pkt.msg.v.serial))
+}
+
+/* Summary of handshake B phase leader */
+predicate Handshake_Leader_PreQuorum_Invariant(tls:TLS_State) 
+    requires DS_Config_Invariant(tls.config, tls)
+    requires ZK_Config_Invariant(tls.config, tls)
+    requires Handshake_Serial_Invariant(tls)
+    requires Quorums_Size_Invariant(tls)
+{
+    var n := |tls.config|;
+    var leaderTQP := tls.t_servers[tls.config[0]];
+    !IsQuorum(n, leaderTQP.v.leader.globals.electingFollowers)
+    ==> 
+    && leaderTQP.ts <= ProcessEpAck_PreQuorum_ts_Formula(tls.f, n, leaderTQP)
+    && leaderTQP.dts <= ProcessEpAck_PreQuorum_dts_Formula(tls.f, n, leaderTQP)
+}
+
+/* Summary of handshake B phase follower */
+predicate Handshake_Follower_Invariant(tls:TLS_State) 
+    requires DS_Config_Invariant(tls.config, tls)
+    requires ZK_Config_Invariant(tls.config, tls)
+{
+    && Follower_HandshakeB_Invariant(tls)
+    && Follower_PreSync_Invariant(tls)
+}
+
+
+/*****************************************************************************************
+*                                 Sync Phase Guarantees                                  *
+*****************************************************************************************/
+
+
+/* For all SyncDIFF | SyncSNAP messages sent */
+function Sync_Message_ts_Formula(f:int, serial:nat) : Timestamp 
+    requires f >= 1;
+{
+    AckEpoch_Message_PreQuorum_ts_Formula(f, f-1)
+    + ProcEpAck * f
+    + ProcEpAck * f
+    + PreSync * f    // max possible PrepSyncs done before I was sent
+    + Sync * serial  // max possible NewLeader sent before I was sent
+    + SyncSnap * (serial + 1)  // I am the (serial + 1)-th sync message sent
+    + D
+}
+
+/* For all NewLeader messages sent */
+function NewLeader_Message_ts_Formula(f:int, serial:nat) : Timestamp 
+    requires f >= 1;
+{
+    AckEpoch_Message_PreQuorum_ts_Formula(f, f-1)
+    + ProcEpAck * f
+    + ProcEpAck * f
+    + PreSync * f    // max possible PrepSyncs done before I was sent
+    + SyncSnap * f  // max possible Syncs sent before I was sent
+    + Sync * (serial + 1)  // I am the (serial + 1)-th NL message sent
+    + D
+}
+
+/* Follower in F_SYNC state. May or may not have received Newleader at this state. 
+* Just received a SyncDiff | SyncSnap | NewLeader */
+function Follower_F_SYNC_dts_Formula(f:int, s:TQuorumPeer) : Timestamp 
+    requires s.v.FollowerPeer?    
+    requires f >= 1
+    requires s.v.follower.serialSync >= 0
+{
+    if s.v.follower.serialNL < 0 
+    then // yet to receive NL. Just processed SyncDiff | SyncSnap
+        Sync_Message_ts_Formula(f, s.v.follower.serialSync)
+    else // just received NL. Waititng to receive final UpToDate to start running
+        NewLeader_Message_ts_Formula(f, s.v.follower.serialNL)
+}
+
+/* Follower in F_SYNC state. May or may not have received Newleader at this state. 
+* Just received a SyncDiff | SyncSnap | NewLeader */
+function Follower_F_SYNC_ts_Formula(f:int, s:TQuorumPeer) : Timestamp 
+    requires s.v.FollowerPeer?    
+    requires f >= 1
+    requires s.v.follower.serialSync >= 0
+{
+    if s.v.follower.serialNL < 0 
+    then // yet to receive NL. Just processed SyncDiff | SyncSnap
+        Follower_F_SYNC_dts_Formula(f, s) + ProcSnap
+    else // just received NL. Waititng to receive final UpToDate to start running
+        NewLeader_Message_ts_Formula(f, f-1) + ProcSnap + ProcSync
+}
+
+
+function Ack_Message_ts_Formula(f:int, serial:nat) : Timestamp
+    requires f >= 1;
+{
+    NewLeader_Message_ts_Formula(f, f-1) + ProcSnap + ProcSync + D
+}
+
+
+function ProcessAck_PreQuorum_ts_Formula(f:int, n:int, l:TQuorumPeer) : Timestamp 
+    requires l.v.LeaderPeer?
+    requires f >= 1
+    requires !IsQuorum(n, l.v.leader.globals.ackSet)
+    requires |l.v.leader.globals.electingFollowers| >= 1;
+{
+    var electingFollowers := l.v.leader.globals.electingFollowers;
+    var ackSet := l.v.leader.globals.ackSet;
+    if |ackSet| <= 1 then 
+        AckEpoch_Message_PreQuorum_ts_Formula(f, f-1)
+        + ProcEpAck * (|electingFollowers|-1)
+        + ProcEpAck * l.v.leader.globals.procEpCount 
+        + PreSync * l.v.leader.globals.prepCount    // num of PrepSyncs done
+        + SyncSnap * l.v.leader.globals.nextSerialSync   // Number of SyncSnaps done
+        + Sync * l.v.leader.globals.nextSerialNL   
+    else 
+        Ack_Message_ts_Formula(f, f-1) + ProcAck * (|ackSet|-1)
+}
+
+
+function ProcessAck_PreQuorum_dts_Formula(f:int, n:int, l:TQuorumPeer) : Timestamp 
+    requires l.v.LeaderPeer?
+    requires f >= 1
+    requires !IsQuorum(n, l.v.leader.globals.ackSet)
+{
+    var ackSet := l.v.leader.globals.ackSet;
+    if |ackSet| <= 1 then 
+        // Have not received any Acks. Dts is from last AckEpoch received
+        // The largest AckEpoch serial I can get is f
+        AckEpoch_Message_PreQuorum_ts_Formula(f, f-1)
+    else 
+        // From the last Ack I received
+        // The largest Ack serial I can get is f
+        Ack_Message_ts_Formula(f, f-1)
+}
+
+
+//----------------------------------------------------------------------------------------
+/* Summary of Sync phase messages */
+predicate Sync_Messages_Invariant(tls:TLS_State) 
+    requires DS_Config_Invariant(tls.config, tls)
+    requires ZK_Config_Invariant(tls.config, tls)
+{   
+    && (forall pkt | pkt in tls.t_environment.sentPackets && (pkt.msg.v.SyncDIFF? || pkt.msg.v.SyncSNAP?) 
+    :: pkt.msg.ts <= Sync_Message_ts_Formula(tls.f, pkt.msg.v.serial))
+    && (forall pkt | pkt in tls.t_environment.sentPackets && pkt.msg.v.NewLeader? 
+    :: pkt.msg.ts <= NewLeader_Message_ts_Formula(tls.f, pkt.msg.v.serial))
+    && (forall pkt | pkt in tls.t_environment.sentPackets && pkt.msg.v.Ack? 
+    :: pkt.msg.ts <= Ack_Message_ts_Formula(tls.f, pkt.msg.v.serial))
+}
+
+
+/* Summary of Sync phase followers */
+predicate Sync_Follower_Invariant(tls:TLS_State){
+    forall ep | 
+        && ep in tls.t_servers
+        && tls.t_servers[ep].v.FollowerPeer? 
+        && tls.t_servers[ep].v.follower.state == F_SYNC
+        && 0 <= tls.t_servers[ep].v.follower.serialSync < tls.f
+    ::  && tls.t_servers[ep].dts <= Follower_F_SYNC_dts_Formula(tls.f, tls.t_servers[ep])
+        && tls.t_servers[ep].ts <= Follower_F_SYNC_ts_Formula(tls.f, tls.t_servers[ep])
+}
+
+
+/* Summary of Sync phase leader before AckSet quorum */
+predicate Sync_Leader_PreQuorum_Invariant(tls:TLS_State) 
+    requires DS_Config_Invariant(tls.config, tls)
+    requires ZK_Config_Invariant(tls.config, tls)
+    requires Quorums_Size_Invariant(tls)
+{
+    var n := |tls.config|;
+    var leaderTQP := tls.t_servers[tls.config[0]];
+    // && IsQuorum(n, leaderTQP.v.leader.globals.electingFollowers)
+    && !IsQuorum(n, leaderTQP.v.leader.globals.ackSet)
+    ==> 
+    && leaderTQP.ts <= ProcessAck_PreQuorum_ts_Formula(tls.f, n, leaderTQP)
+    && leaderTQP.dts <= ProcessAck_PreQuorum_dts_Formula(tls.f, n, leaderTQP)
+}
+
+
+/*****************************************************************************************
+*                          Some lemmas comparing timestamps                              *
+*****************************************************************************************/
+
+}
