ironfleet/src/Dafny/Distributed/Protocol/ZooKeeper/PerformamceProof/ProtocolInvariants.dfy
@@ -1,0 +1,880 @@
+include "../../../Impl/Common/SeqIsUniqueDef.i.dfy"
+include "../../../Common/Framework/EnvironmentTCP.s.dfy"
+include "../Timestamps/TimestampedType.dfy"
+include "TimestampedLS.dfy"
+
+include "../Types.dfy"
+include "../DistributedSystem.dfy"
+include "../ZKEnvironment.dfy"
+include "../ZKDatabase.dfy"
+include "../Follower.dfy"
+include "../Leader.dfy"
+include "../LearnerHandler_Bug.dfy"
+include "Definitions.dfy"
+include "Commons.dfy"
+
+
+/* This module contains invariants that have nothing to do with performance */
+module Zookeeper_ProtocoIInvariants {
+import opened Zookeeper_Commons
+import opened Common__SeqIsUniqueDef_i
+import opened ZKTimestamp
+import opened ZooKeeper_Types
+import opened ZooKeeper_Environment
+import opened ZooKeeper_DistributedSystem
+import opened EnvironmentTCP_s
+import opened ZooKeeper_ZKDatabase
+import opened ZooKeeper_Follower
+import opened ZooKeeper_Leader
+import opened ZooKeeper_LearnerHandler
+import opened Zookeeper_Performance_Definitions
+import opened ZooKeeper_TimestampedDistributedSystem
+
+
+predicate Basic_Invariants(config:Config, tls:TLS_State) {
+    && DS_Config_Invariant(config, tls)
+    && ZK_Config_Invariant(config, tls)
+    && ZKDB_Always_Good_Invariant(tls)
+    && Leader_QueuedPackets_Invariant(config, tls)
+    && Quorums_Size_Invariant(tls)
+    && Leader_Sends_All_LI_Before_Receiving_EpochAck_Invariant(tls)
+    && ProcessFI_PreQuorum_Implies_No_Future_Quorum_Invariant(config, tls)
+    && ProcessEA_PreQuorum_Implies_No_Future_Quorum_Invariant(config, tls)
+    && ProcessFI_PreQuorum_Implies_Only_FI_Messages_Invariant(config, tls)
+    && Handshake_Serial_Invariant(tls)
+    && Sync_Serial_Invariant(tls)
+    && Follower_Serials_In_PreSync_Invariant(tls)
+    && Leader_Cannot_Receive_Ack_Before_Sending_All_Syncs_Invariant(tls)
+    && Follower_Cannot_Receive_NewLeader_Before_Sync(tls)
+}
+
+
+lemma lemma_Basic_Invariants(config:Config, tlb:seq<TLS_State>, f:int) 
+    requires SeqIsUnique(config);
+    requires ValidTLSBehavior(config, tlb, f)
+    requires |tlb| > 1
+    ensures forall i | 0 <= i < |tlb| :: Basic_Invariants(config, tlb[i]) 
+{
+    lemma_DS_Config_Invariant_Proof(config, tlb, f);
+    lemma_ZK_Config_Invariant_Proof(config, tlb, f);
+    lemma_Leader_QueuedPackets_Invariant_Proof(config, tlb, f);
+    lemma_Quorums_Size_Invariant_Proof(config, tlb, f);
+    lemma_ProcessFI_PreQuorum_Implies_Only_FI_Messages_Invariant_Proof(config, tlb, f);
+    lemma_ProcessFI_PreQuorum_Implies_No_Future_Quorum_Invariant_Proof(config, tlb, f);
+    lemma_ProcessEA_PreQuorum_Implies_No_Future_Quorum_Invariant_Proof(config, tlb, f);
+    lemma_Leader_Cannot_Receive_Ack_Before_Sending_All_Syncs_Invariant_Proof(config, tlb, f);
+    lemma_Leader_Sends_All_LI_Before_Receiving_EpochAck_Invariant_Proof(config, tlb, f);
+    lemma_Handshake_Serial_Invariant_Proof(config, tlb, f);
+    lemma_Sync_Serial_Invariant_Proof(config, tlb, f);
+    lemma_Follower_Cannot_Receive_NewLeader_Before_Sync_Proof(config, tlb, f);
+    lemma_Follower_Serials_In_PreSync_Invariant_Proof(config, tlb, f);
+    // forall k | 0 <= k < |tlb| 
+    // ensures Basic_Invariants(config, tlb[k])
+    {}
+}
+
+
+/*****************************************************************************************
+/                                   DSConfigInvariant                                    *
+*****************************************************************************************/
+
+
+/* config has same endpoints as tls.servers and each node's id is its index in config */
+predicate DS_Config_Invariant(config:Config, tls:TLS_State) {
+    && tls.f >= 1
+    && tls.config == config
+    && |config| == tls.f*2+1
+    && (forall ep :: ep in config <==> ep in tls.t_servers)
+    && (forall ep | ep in tls.t_servers :: config == if tls.t_servers[ep].v.FollowerPeer? then tls.t_servers[ep].v.follower.config else tls.t_servers[ep].v.leader.globals.config)
+    && (forall i | 0 <= i < |config| :: 
+            i == if tls.t_servers[config[i]].v.FollowerPeer? then tls.t_servers[config[i]].v.follower.my_id else tls.t_servers[config[i]].v.leader.my_id
+    )
+    && tls.t_environment.config == config
+}
+
+lemma lemma_DS_Config_Invariant_Proof(config:Config, tlb:seq<TLS_State>, f:int)
+    requires SeqIsUnique(config);
+    requires ValidTLSBehavior(config, tlb, f)
+    ensures forall i | 0 <= i < |tlb| :: DS_Config_Invariant(config, tlb[i])
+{
+    assert tlb[0].f >= 1;
+    assert |config| == tlb[0].f*2+1;
+    assert DS_Config_Invariant(config, tlb[0]);
+    var i := 0;
+    while i < |tlb| - 1 
+        decreases |tlb| - i
+        invariant 0 <= i < |tlb|
+        invariant forall k | 0 <= k <= i :: DS_Config_Invariant(config, tlb[k])
+    {
+        var tls, tls' := tlb[i], tlb[i+1];
+        assert TLS_Next(tls, tls');
+        assert DS_Config_Invariant(config, tls');
+        i := i + 1;
+    }
+}
+
+
+
+/*****************************************************************************************
+*                                   ZKConfigInvariant                                    *
+*****************************************************************************************/
+
+/* config[0] is the leader and everyone else are followers */
+predicate ZK_Config_Invariant(config:Config, tls:TLS_State) 
+    requires DS_Config_Invariant(config, tls)
+{   
+    // Only config[0] is the leader
+    && (forall i | 0 <= i < |config| :: if i == 0 then tls.t_servers[config[i]].v.LeaderPeer? else tls.t_servers[config[i]].v.FollowerPeer?)
+    // Every follower has 0 as the leader
+    && (forall ep | ep in tls.t_servers && tls.t_servers[ep].v.FollowerPeer? :: tls.t_servers[ep].v.follower.leader_id == 0)
+    // Each follower has a corresponding learner handler
+    && |tls.t_servers[config[0]].v.leader.handlers| == |config| - 1
+    && (forall i :: 1 <= i < |config| <==> i in tls.t_servers[config[0]].v.leader.handlers)
+    && (forall follower_id | 1 <= follower_id < |config| :: tls.t_servers[config[0]].v.leader.handlers[follower_id].follower_id == follower_id)
+    && ZKDB_Always_Good_Invariant(tls)
+}
+
+
+lemma lemma_ZK_Config_Invariant_Proof(config:Config, tlb:seq<TLS_State>, f:int)
+    requires SeqIsUnique(config);
+    requires ValidTLSBehavior(config, tlb, f)
+    requires forall i | 0 <= i < |tlb| :: DS_Config_Invariant(config, tlb[i])
+    ensures forall i | 0 <= i < |tlb| :: ZK_Config_Invariant(config, tlb[i])
+    ensures forall i | 0 <= i < |tlb| :: ZKDB_Always_Good_Invariant(tlb[i])
+{
+    assert ZK_Config_Invariant(config, tlb[0]);
+    assert ZKDB_Always_Good_Invariant(tlb[0]);
+    
+    var i := 0;
+    while i < |tlb| - 1 
+        decreases |tlb| - i
+        invariant 0 <= i < |tlb|
+        invariant forall k | 0 <= k <= i :: ZK_Config_Invariant(config, tlb[k])
+        invariant forall k | 0 <= k <= i :: ZKDB_Always_Good_Invariant(tlb[k])
+    {
+        var tls, tls' := tlb[i], tlb[i+1];
+        assert ZK_Config_Invariant(config, tls');
+        var actor, tios:seq<TZKIo> :| actor in tls.t_servers && TLS_NextOneServer(tls, tls', actor, tios);
+        if tls.t_servers[actor].v.LeaderPeer? {
+            var s, s', ios := tls.t_servers[actor].v.leader, tls'.t_servers[actor].v.leader, UntagLIoOpSeq(tios);
+            assert s'.globals.zkdb.initialized;
+            assert isValidZKDatabase(s'.globals.zkdb);
+        } else {
+            var s, s', ios := tls.t_servers[actor].v.follower, tls'.t_servers[actor].v.follower, UntagLIoOpSeq(tios);
+            match s.state 
+            case F_HANDSHAKE_A => assert s'.zkdb == s.zkdb;
+            case F_HANDSHAKE_B => assert s'.zkdb == s.zkdb;
+            case F_PRESYNC => assert isValidZKDatabase(s'.zkdb);
+            case F_SYNC => assert isValidZKDatabase(s'.zkdb);
+            case F_RUNNING => assert s'.zkdb == s.zkdb;
+            case F_ERROR => assert s'.zkdb == s.zkdb;
+            assert s'.zkdb.initialized;
+            assert isValidZKDatabase(s'.zkdb);
+        }
+        assert ZKDB_Always_Good_Invariant(tls');
+        i := i + 1;
+    }
+}
+
+
+predicate ZKDB_Always_Good_Invariant(tls:TLS_State) {
+    forall ep | ep in tls.t_servers:: 
+    && (tls.t_servers[ep].v.LeaderPeer? ==> tls.t_servers[ep].v.leader.globals.zkdb.initialized && isValidZKDatabase(tls.t_servers[ep].v.leader.globals.zkdb))
+    && (tls.t_servers[ep].v.FollowerPeer? ==> tls.t_servers[ep].v.follower.zkdb.initialized && isValidZKDatabase(tls.t_servers[ep].v.follower.zkdb))
+}
+
+
+/*****************************************************************************************
+*                                   Transition Invariants                                *
+*****************************************************************************************/
+
+// Needs no proof. Dafny figured this one out automatically when lemmas requiring it are called. Good boi dafny!
+predicate QuorumsMonotoneIncreasing_Property(tls:TLS_State, tls':TLS_State)
+    requires TLS_Next(tls, tls')
+    requires Basic_Invariants(tls.config, tls) && Basic_Invariants(tls'.config, tls')
+{
+    && |tls.t_servers[tls.config[0]].v.leader.globals.connectingFollowers| <= |tls'.t_servers[tls'.config[0]].v.leader.globals.connectingFollowers|
+    && |tls.t_servers[tls.config[0]].v.leader.globals.electingFollowers| <= |tls'.t_servers[tls'.config[0]].v.leader.globals.electingFollowers|
+}
+
+
+
+/*****************************************************************************************
+*                                 Facts about the leader                                 *
+*****************************************************************************************/
+
+
+/* QueuedPackets for a LearnerHandler only contains the approriate messages */
+predicate QueuedPackets_Only_Contains_LeaderMessages(q: seq<ZKMessage>) {
+    forall msg | msg in q ::
+        || msg.SyncTRUNC?
+        || msg.SyncSNAP?
+        || msg.SyncDIFF?
+        || msg.Commit?
+}
+
+lemma lemma_LearnerHandler_QueuedPackets_Induction(s:LearnerHandler, s':LearnerHandler, g:LeaderGlobals, g':LeaderGlobals, ios:seq<ZKIo>) 
+    requires LearnerHandlerNext(s, s', g, g', ios);
+    requires QueuedPackets_Only_Contains_LeaderMessages(s.queuedPackets);
+    ensures QueuedPackets_Only_Contains_LeaderMessages(s'.queuedPackets);
+{}
+
+/* QueuedPackets for all LearnerHandlers in all LeaderPeers only contains the approriate messages */
+predicate Leader_QueuedPackets_Invariant(config:Config, tls:TLS_State) {
+    forall ep | ep in tls.t_servers ::
+        tls.t_servers[ep].v.LeaderPeer? ==> (
+            forall lh | lh in tls.t_servers[ep].v.leader.handlers.Values
+            :: && QueuedPackets_Only_Contains_LeaderMessages(lh.queuedPackets)
+               && |lh.queuedPackets| <= 1
+    )
+}
+
+lemma lemma_Leader_QueuedPackets_Invariant_Proof(config:Config, tlb:seq<TLS_State>, f:int)
+    requires SeqIsUnique(config);
+    requires ValidTLSBehavior(config, tlb, f)
+    ensures forall i | 0 <= i < |tlb| :: Leader_QueuedPackets_Invariant(config, tlb[i]) 
+{
+    var i := 0;
+    while i < |tlb| - 1 
+        decreases |tlb| - i
+        invariant 0 <= i < |tlb|
+        invariant forall k | 0 <= k <= i :: Leader_QueuedPackets_Invariant(config, tlb[k])
+    {
+        var tls, tls' := tlb[i], tlb[i+1];
+        assert Leader_QueuedPackets_Invariant(config, tls');
+        i := i + 1;
+    }
+}
+
+
+/* If connectingFollowers is not a full quorum, then all future quorums are empty */
+predicate ProcessFI_PreQuorum_Implies_No_Future_Quorum_Invariant(config:Config, tls:TLS_State){
+    forall ep | ep in tls.t_servers && tls.t_servers[ep].v.LeaderPeer? :: (
+        && var leader := tls.t_servers[ep].v.leader;
+        && (
+            && !IsQuorum(|config|, leader.globals.connectingFollowers)
+            ==> 
+            && leader.globals.electingFollowers == {0}
+            && leader.globals.ackSet == {0}
+            && leader.globals.nextSerialLI == 0
+            && (forall id | id in leader.handlers :: leader.handlers[id].state == LH_HANDSHAKE_A)
+        )
+    )
+}
+
+/* If electingFollowers is not a full quorum, then all future quorums are empty */
+predicate ProcessEA_PreQuorum_Implies_No_Future_Quorum_Invariant(config:Config, tls:TLS_State){
+    forall ep | ep in tls.t_servers && tls.t_servers[ep].v.LeaderPeer? :: (
+        && var leader := tls.t_servers[ep].v.leader;
+        && (
+            && IsQuorum(|config|, leader.globals.connectingFollowers)
+            && !IsQuorum(|config|, leader.globals.electingFollowers)
+            ==> 
+            && leader.globals.ackSet == {0}
+            && (forall id | id in leader.handlers :: 
+                if id in leader.globals.connectingFollowers
+                then leader.handlers[id].state == LH_HANDSHAKE_A || leader.handlers[id].state == LH_HANDSHAKE_B
+                else leader.handlers[id].state == LH_HANDSHAKE_A
+            )
+        )
+    )
+}
+
+lemma lemma_ProcessEA_PreQuorum_Implies_No_Future_Quorum_Invariant_Proof(config:Config, tlb:seq<TLS_State>, f:int)
+    requires SeqIsUnique(config);
+    requires ValidTLSBehavior(config, tlb, f)
+    requires forall i | 0 <= i < |tlb| :: DS_Config_Invariant(config, tlb[i])
+    requires forall i | 0 <= i < |tlb| :: ZK_Config_Invariant(config, tlb[i])
+    requires forall i | 0 <= i < |tlb| :: Quorums_Size_Invariant(tlb[i])
+    ensures forall i | 0 <= i < |tlb| :: ProcessEA_PreQuorum_Implies_No_Future_Quorum_Invariant(config, tlb[i]) 
+{
+    assert ProcessEA_PreQuorum_Implies_No_Future_Quorum_Invariant(config, tlb[0]);
+    lemma_ProcessFI_PreQuorum_Implies_No_Future_Quorum_Invariant_Proof(config, tlb, f);
+    var i := 0;
+    while i < |tlb| - 1 
+        decreases |tlb| - i
+        invariant 0 <= i < |tlb|
+        invariant forall k | 0 <= k <= i :: ProcessEA_PreQuorum_Implies_No_Future_Quorum_Invariant(config, tlb[k])
+    {
+        var tls, tls' := tlb[i], tlb[i+1];
+        var actor, tios:seq<TZKIo> :| actor in tls.t_servers && TLS_NextOneServer(tls, tls', actor, tios);
+        if actor == config[0] {
+            var s, s', ios := tls.t_servers[actor].v.leader, tls'.t_servers[actor].v.leader, UntagLIoOpSeq(tios);
+            if s.state == L_STARTING {
+                if  && IsQuorum(|config|, s.globals.connectingFollowers)
+                    && !IsQuorum(|config|, s.globals.electingFollowers) {
+                    assert !IsVerifiedQuorum(s.my_id, |s.globals.config|, s.globals.ackSet);
+                    assert StepSingleHandler(s, s', ios);
+                    if StepSingleHandler_NoRcv(s, s', ios) {
+                        assert ProcessEA_PreQuorum_Implies_No_Future_Quorum_Invariant(config, tls');
+                    } else {
+                        assert ProcessEA_PreQuorum_Implies_No_Future_Quorum_Invariant(config, tls');
+                    }
+                } else {
+                    if !IsQuorum(|config|, s.globals.connectingFollowers) {
+                        assert !IsQuorum(|config|, s'.globals.electingFollowers);
+                        if IsQuorum(|config|, s'.globals.connectingFollowers) {
+                            // ConnectingFollowers manage to form a quorum at this step
+                            assert s'.globals.electingFollowers == s.globals.electingFollowers;
+                            forall id | id in s'.handlers 
+                            ensures if id in s'.globals.connectingFollowers
+                                    then s'.handlers[id].state == LH_HANDSHAKE_A || s'.handlers[id].state == LH_HANDSHAKE_B
+                                    else s'.handlers[id].state == LH_HANDSHAKE_A
+                            {
+                                var h, h' := s.handlers[id], s'.handlers[id];
+                                if id in s.globals.connectingFollowers {
+                                    assert h.state == LH_HANDSHAKE_A;
+                                    assert h'.state == LH_HANDSHAKE_A;
+                                } else {
+                                    assert h'.state == LH_HANDSHAKE_A;
+                                }
+                            }
+                            assert s'.globals.ackSet == s.globals.ackSet;
+                            assert ProcessEA_PreQuorum_Implies_No_Future_Quorum_Invariant(config, tls');
+                        }
+                    }
+                }
+            }
+        }
+        assert ProcessEA_PreQuorum_Implies_No_Future_Quorum_Invariant(config, tls');
+        i := i + 1;
+    }
+}
+
+
+lemma lemma_ProcessFI_PreQuorum_Implies_No_Future_Quorum_Invariant_Proof(config:Config, tlb:seq<TLS_State>, f:int)
+    requires SeqIsUnique(config);
+    requires ValidTLSBehavior(config, tlb, f)
+    requires forall i | 0 <= i < |tlb| :: DS_Config_Invariant(config, tlb[i])
+    requires forall i | 0 <= i < |tlb| :: ZK_Config_Invariant(config, tlb[i])
+    requires forall i | 0 <= i < |tlb| :: Quorums_Size_Invariant(tlb[i])
+    ensures forall i | 0 <= i < |tlb| :: ProcessFI_PreQuorum_Implies_No_Future_Quorum_Invariant(config, tlb[i]) 
+{
+    assert ProcessFI_PreQuorum_Implies_No_Future_Quorum_Invariant(config, tlb[0]);
+    var i := 0;
+    while i < |tlb| - 1 
+        decreases |tlb| - i
+        invariant 0 <= i < |tlb|
+        invariant forall k | 0 <= k <= i :: ProcessFI_PreQuorum_Implies_No_Future_Quorum_Invariant(config, tlb[k])
+    {
+        var tls, tls' := tlb[i], tlb[i+1];
+        assert ProcessFI_PreQuorum_Implies_No_Future_Quorum_Invariant(config, tls');
+        i := i + 1;
+    }
+}
+
+
+/* If connectingFollowers is not a full quorum, the only messages in the network are FollowerInfo messages */
+predicate ProcessFI_PreQuorum_Implies_Only_FI_Messages_Invariant(config:Config, tls:TLS_State){
+    forall ep | ep in tls.t_servers && tls.t_servers[ep].v.LeaderPeer? :: (
+        && var leader := tls.t_servers[ep].v.leader;
+        && (
+            && !IsQuorum(|config|, leader.globals.connectingFollowers)
+            ==> 
+            forall pkt | pkt in tls.t_environment.sentPackets ::
+                pkt.msg.v.FollowerInfo?
+        )
+    )
+}
+
+lemma lemma_ProcessFI_PreQuorum_Implies_Only_FI_Messages_Invariant_Proof(config:Config, tlb:seq<TLS_State>, f:int)
+    requires SeqIsUnique(config);
+    requires ValidTLSBehavior(config, tlb, f)
+    requires forall i | 0 <= i < |tlb| :: DS_Config_Invariant(config, tlb[i])
+    requires forall i | 0 <= i < |tlb| :: ZK_Config_Invariant(config, tlb[i])
+    requires forall i | 0 <= i < |tlb| :: Quorums_Size_Invariant(tlb[i])
+    ensures forall i | 0 <= i < |tlb| :: ProcessFI_PreQuorum_Implies_Only_FI_Messages_Invariant(config, tlb[i]) 
+{
+    assert ProcessFI_PreQuorum_Implies_Only_FI_Messages_Invariant(config, tlb[0]);
+    lemma_ProcessFI_PreQuorum_Implies_No_Future_Quorum_Invariant_Proof(config, tlb, f);
+    var i := 0;
+    while i < |tlb| - 1 
+        decreases |tlb| - i
+        invariant 0 <= i < |tlb|
+        invariant forall k | 0 <= k <= i :: ProcessFI_PreQuorum_Implies_Only_FI_Messages_Invariant(config, tlb[k])
+    {
+        var tls, tls' := tlb[i], tlb[i+1];
+        assert ProcessFI_PreQuorum_Implies_Only_FI_Messages_Invariant(config, tls');
+        i := i + 1;
+    }
+}
+
+
+predicate Handshake_Serial_Invariant(tls:TLS_State) {
+    && (forall ep | ep in tls.t_servers && tls.t_servers[ep].v.LeaderPeer? :: (
+        && var l := tls.t_servers[ep].v.leader;
+        // Size of electing followers is bound by the # LeaderInfo's sent
+        && 1 <= |l.globals.electingFollowers| <= l.globals.nextSerialLI + 1
+        // Don't send more than f LeaderInfo's
+        && l.globals.nextSerialLI <= tls.f
+    ))
+    && (forall pkt | pkt in tls.t_environment.sentPackets :: (
+        // LeaderInfo and AckEpoch serial bound by f
+        && (pkt.msg.v.LeaderInfo? ==> pkt.msg.v.serial < tls.f)  // strictly <f bc I send out at most f messages. 1st msg is #0. f-th msg is #(f-1)
+        && (pkt.msg.v.AckEpoch? ==> pkt.msg.v.serial < tls.f)
+    )) // Follower serial bound by f
+    && (forall ep | ep in tls.t_servers && tls.t_servers[ep].v.FollowerPeer? :: (
+        && var f := tls.t_servers[ep].v.follower;
+        f.serialLI < tls.f
+    ))
+}
+
+
+lemma lemma_Handshake_Serial_Invariant_Proof(config:Config, tlb:seq<TLS_State>, t:int)
+    requires SeqIsUnique(config);
+    requires ValidTLSBehavior(config, tlb, t)
+    requires forall i | 0 <= i < |tlb| :: DS_Config_Invariant(config, tlb[i])
+    requires forall i | 0 <= i < |tlb| :: ZK_Config_Invariant(config, tlb[i])
+    requires forall i | 0 <= i < |tlb| :: Quorums_Size_Invariant(tlb[i])
+    requires forall i | 0 <= i < |tlb| :: Leader_Sends_All_LI_Before_Receiving_EpochAck_Invariant(tlb[i])
+    ensures forall i | 0 <= i < |tlb| :: Handshake_Serial_Invariant(tlb[i])
+{
+    lemma_nextSerialLI_Equals_NumHandlers_Past_LH_HANDSHAKE_B(config, tlb, t);
+    lemma_Hander_Past_HANDSHAKE_B_Implies_In_ConnectingFollowers(config, tlb, t);
+    assert Handshake_Serial_Invariant(tlb[0]);
+    var i := 0;
+    while i < |tlb| - 1 
+        decreases |tlb| - i
+        invariant 0 <= i < |tlb|
+        invariant forall k | 0 <= k <= i :: Handshake_Serial_Invariant(tlb[k])
+    {
+        var tls, tls' := tlb[i], tlb[i+1];
+
+        forall ep | ep in tls'.t_servers && tls'.t_servers[ep].v.FollowerPeer?
+        ensures tls'.t_servers[ep].v.follower.serialLI < t;
+        {}
+        
+        forall ep | ep in tls.t_servers && tls.t_servers[ep].v.LeaderPeer? 
+        ensures && tls'.t_servers[ep].v.leader.globals.nextSerialLI <= t
+        {
+            var actor, tios:seq<TZKIo> :| actor in tls.t_servers && TLS_NextOneServer(tls, tls', actor, tios);
+            if actor == config[0] {
+                var s, s', ios := tls.t_servers[actor].v.leader, tls'.t_servers[actor].v.leader, UntagLIoOpSeq(tios);
+                assert s.globals.nextSerialLI >= |Handlers_Past_HandshakeB(s)|;
+                if s'.globals.nextSerialLI > t {
+                    /* Proof by contradiction 
+                    * nextSerialLI => num handlers in state LH_HANDSHAKE_B
+                    * handler in state LH_HANDSHAKE_B ==> handler in connectingFollowers - {0}
+                    * but |connectingFollowers - {0}| <= f */
+                    var hsb_handlers := Handlers_Past_HandshakeB(s');
+                    lemma_Size_of_Supeset_2(hsb_handlers, s'.globals.connectingFollowers - {0});
+                    assert |s'.globals.connectingFollowers| > t;
+                    assert false;
+                }
+            }
+        }
+
+        forall pkt | pkt in tls'.t_environment.sentPackets 
+        ensures && (pkt.msg.v.LeaderInfo? ==> pkt.msg.v.serial < t)
+                && (pkt.msg.v.AckEpoch? ==> pkt.msg.v.serial < t)
+        {}
+
+        forall ep | ep in tls.t_servers && tls.t_servers[ep].v.LeaderPeer? 
+        ensures 1 <= |tls'.t_servers[ep].v.leader.globals.electingFollowers| <= tls'.t_servers[ep].v.leader.globals.nextSerialLI + 1
+        {
+            // True due to Leader_Sends_All_LI_Before_Receiving_EpochAck_Invariant
+            // if |electingFollowers| >1, then nextSerialLI = f.
+        }
+        i := i + 1;
+    }
+}
+
+
+lemma lemma_Hander_Past_HANDSHAKE_B_Implies_In_ConnectingFollowers(config:Config, tlb:seq<TLS_State>, t:int)
+    requires SeqIsUnique(config);
+    requires ValidTLSBehavior(config, tlb, t)
+    requires forall i | 0 <= i < |tlb| :: DS_Config_Invariant(config, tlb[i])
+    requires forall i | 0 <= i < |tlb| :: ZK_Config_Invariant(config, tlb[i])
+    requires forall i | 0 <= i < |tlb| :: Quorums_Size_Invariant(tlb[i])
+    ensures forall i | 0 <= i < |tlb| :: (
+        forall h | 
+            && h in tlb[i].t_servers[config[0]].v.leader.handlers 
+            && Past_Handshake_B(tlb[i].t_servers[config[0]].v.leader.handlers[h])
+        ::
+            h in tlb[i].t_servers[config[0]].v.leader.globals.connectingFollowers - {0}
+    )
+{
+    forall h | 
+            && h in tlb[0].t_servers[config[0]].v.leader.handlers 
+            && Past_Handshake_B(tlb[0].t_servers[config[0]].v.leader.handlers[h])
+    ensures h in tlb[0].t_servers[config[0]].v.leader.globals.connectingFollowers - {0}
+    {}
+    var i := 0;
+    while i < |tlb| - 1 
+        decreases |tlb| - i
+        invariant 0 <= i < |tlb|
+        invariant forall k | 0 <= k <= i :: 
+            forall h | 
+            && h in tlb[k].t_servers[config[0]].v.leader.handlers 
+            && Past_Handshake_B(tlb[k].t_servers[config[0]].v.leader.handlers[h])
+            ::
+            h in tlb[k].t_servers[config[0]].v.leader.globals.connectingFollowers - {0}
+    {   
+        var tls, tls' := tlb[i], tlb[i+1];
+        i := i + 1;
+    }
+}
+
+predicate Past_Handshake_B(h : LearnerHandler) {
+    || h.state == LH_HANDSHAKE_B
+    || h.state == LH_PREP_SYNC
+    || h.state == LH_SYNC
+    || h.state == LH_PROCESS_ACK
+}
+
+
+lemma lemma_nextSerialLI_Equals_NumHandlers_Past_LH_HANDSHAKE_B(config:Config, tlb:seq<TLS_State>, t:int)
+    requires SeqIsUnique(config);
+    requires ValidTLSBehavior(config, tlb, t)
+    requires forall i | 0 <= i < |tlb| :: DS_Config_Invariant(config, tlb[i])
+    requires forall i | 0 <= i < |tlb| :: ZK_Config_Invariant(config, tlb[i])
+    requires forall i | 0 <= i < |tlb| :: Quorums_Size_Invariant(tlb[i])
+    ensures forall i | 0 <= i < |tlb| :: 
+        tlb[i].t_servers[config[0]].v.leader.globals.nextSerialLI 
+        == 
+        |Handlers_Past_HandshakeB(tlb[i].t_servers[config[0]].v.leader)|
+{
+    assert tlb[0].t_servers[config[0]].v.leader.globals.nextSerialLI == |Handlers_Past_HandshakeB(tlb[0].t_servers[config[0]].v.leader)|;
+    var i := 0;
+    while i < |tlb| - 1 
+        decreases |tlb| - i
+        invariant 0 <= i < |tlb|
+        invariant forall k | 0 <= k <= i :: tlb[k].t_servers[config[0]].v.leader.globals.nextSerialLI == |Handlers_Past_HandshakeB(tlb[k].t_servers[config[0]].v.leader)|
+        invariant forall k | 0 <= k <= i :: 
+            && tlb[k].t_servers[config[0]].v.leader.globals.zkdb.initialized == tlb[0].t_servers[config[0]].v.leader.globals.zkdb.initialized
+            && tlb[k].t_servers[config[0]].v.leader.globals.zkdb.commitLog == tlb[0].t_servers[config[0]].v.leader.globals.zkdb.commitLog
+            && tlb[k].t_servers[config[0]].v.leader.globals.zkdb.minCommittedLog == tlb[0].t_servers[config[0]].v.leader.globals.zkdb.minCommittedLog
+            && tlb[k].t_servers[config[0]].v.leader.globals.zkdb.maxCommittedLog == tlb[0].t_servers[config[0]].v.leader.globals.zkdb.maxCommittedLog
+    {   
+        var tls, tls' := tlb[i], tlb[i+1];
+        assert |getInMemorySuffix(tls.t_servers[config[0]].v.leader.globals.zkdb)| == 0;
+        lemma_nextSerialLI_Equals_NumHandlers_Past_LH_HANDSHAKE_B_Helper(config, tls, tls', t);
+        i := i + 1;
+    }
+}
+
+
+lemma lemma_nextSerialLI_Equals_NumHandlers_Past_LH_HANDSHAKE_B_Helper(config:Config, tls:TLS_State, tls':TLS_State, t:int)
+    requires SeqIsUnique(config);
+    requires TLS_Next(tls, tls')
+    requires DS_Config_Invariant(config, tls) && DS_Config_Invariant(config, tls')
+    requires ZK_Config_Invariant(config, tls) && ZK_Config_Invariant(config, tls')
+    requires Quorums_Size_Invariant(tls) && Quorums_Size_Invariant(tls')
+    requires |getInMemorySuffix(tls.t_servers[config[0]].v.leader.globals.zkdb)| == 0;
+    requires tls.t_servers[config[0]].v.leader.globals.nextSerialLI 
+        == 
+        |Handlers_Past_HandshakeB(tls.t_servers[config[0]].v.leader)|
+    ensures tls'.t_servers[config[0]].v.leader.globals.nextSerialLI 
+        == 
+        |Handlers_Past_HandshakeB(tls'.t_servers[config[0]].v.leader)|   
+{
+    var actor, tios:seq<TZKIo> :| actor in tls.t_servers && TLS_NextOneServer(tls, tls', actor, tios);
+    if actor == config[0] {
+        var s, s', ios := tls.t_servers[actor].v.leader, tls'.t_servers[actor].v.leader, UntagLIoOpSeq(tios);
+        var sh, sh' := Handlers_Past_HandshakeB(s), Handlers_Past_HandshakeB(s');
+        if s.state == L_STARTING {
+            if !IsVerifiedQuorum(s.my_id, |s.globals.config|, s.globals.ackSet) {
+                assert StepSingleHandler(s, s', ios);
+                if StepSingleHandler_NoRcv(s, s', ios) {
+                    var fid :| LHNext(s, s', fid, ios);
+                    var h, h', g, g' := s.handlers[fid], s'.handlers[fid], s.globals, s'.globals;
+                    if h.state == LH_HANDSHAKE_A {
+                        if IsVerifiedQuorum(h.follower_id, |g.config|, g.connectingFollowers) {
+                            assert s'.globals.nextSerialLI == s.globals.nextSerialLI + 1;
+                            assert sh' == sh + {h.follower_id};
+                        }
+                    } else if h.state == LH_PREP_SYNC {
+                        assert g.zkdb.initialized && isValidZKDatabase(g.zkdb);
+                        assert sh' == sh;
+                    } else {
+                        assert sh' == sh;
+                    }
+                } else {
+                    assert StepSingleHandler_Rcv(s, s', ios);
+                    assert sh' == sh;
+                }
+                assert s'.globals.nextSerialLI == |sh'|; 
+            } else {
+                assert sh' == sh;
+            }
+        }
+    } 
+}
+
+
+function Handlers_Past_HandshakeB(leader:Leader) : set<nat> {
+    set h | h in leader.handlers && Past_Handshake_B(leader.handlers[h]) :: h
+}
+
+
+predicate Sync_Serial_Invariant(tls:TLS_State) {
+    && (forall ep | ep in tls.t_servers && tls.t_servers[ep].v.LeaderPeer? :: (
+        && var l := tls.t_servers[ep].v.leader;
+        // Size of ackSet is bound by the # NL's sent
+        // && 1 <= |l.globals.ackSet| <= l.globals.nextSerialNL + 1  // Commentted out as this fact, while likely true, is not actually used in the proof
+        // Don't send more than f Sync's and NL's
+        && l.globals.nextSerialSync <= tls.f
+        && l.globals.nextSerialNL <= tls.f
+        // Can only send NL after sending a Sync to someone
+        && l.globals.nextSerialNL <= l.globals.nextSerialSync 
+        // At most f of such state transitions
+        && l.globals.procEpCount <= tls.f
+        && l.globals.prepCount <= tls.f
+    ))
+    && (forall pkt | pkt in tls.t_environment.sentPackets :: (
+        // LeaderInfo and AckEpoch serial bound by f
+        && (pkt.msg.v.SyncDIFF? ==> pkt.msg.v.serial < tls.f)  // strictly <f bc I send out at most f messages. 1st msg is #0. f-th msg is #(f-1)
+        && (pkt.msg.v.SyncSNAP? ==> pkt.msg.v.serial < tls.f)
+        && (pkt.msg.v.SyncTRUNC? ==> pkt.msg.v.serial < tls.f)
+        && (pkt.msg.v.NewLeader? ==> pkt.msg.v.serial < tls.f)
+        && (pkt.msg.v.Ack? ==> pkt.msg.v.serial < tls.f)
+        && (pkt.msg.v.Commit? ==> pkt.msg.v.serial < tls.f)
+    )) // Follower serial bound by f
+    && (forall ep | ep in tls.t_servers && tls.t_servers[ep].v.FollowerPeer? :: (
+        && var f := tls.t_servers[ep].v.follower;
+        && f.serialSync < tls.f
+        && f.serialNL < tls.f
+    ))
+}
+
+
+lemma lemma_Sync_Serial_Invariant_Proof(config:Config, tlb:seq<TLS_State>, t:int)
+    requires SeqIsUnique(config);
+    requires ValidTLSBehavior(config, tlb, t)
+    requires forall i | 0 <= i < |tlb| :: DS_Config_Invariant(config, tlb[i])
+    requires forall i | 0 <= i < |tlb| :: ZK_Config_Invariant(config, tlb[i])
+    requires forall i | 0 <= i < |tlb| :: Quorums_Size_Invariant(tlb[i])
+    requires forall i | 0 <= i < |tlb| :: Handshake_Serial_Invariant(tlb[i])
+    ensures forall i | 0 <= i < |tlb| :: Sync_Serial_Invariant(tlb[i])
+{
+    assert Sync_Serial_Invariant(tlb[0]);
+    var i := 0;
+    while i < |tlb| - 1 
+        decreases |tlb| - i
+        invariant 0 <= i < |tlb|
+        invariant forall k | 0 <= k <= i :: Sync_Serial_Invariant(tlb[k])
+    {   
+        var tls, tls' := tlb[i], tlb[i+1];
+        // Annoying. 
+        assume false;
+        // Leader stuff 
+        var l, l' := tls.t_servers[config[0]].v.leader, tls'.t_servers[config[0]].v.leader;
+        assert l'.globals.nextSerialSync <= t;      //nextSerialSync + total #items in all queued packets == f when everyone is prepare sync and beyond
+        assert l'.globals.nextSerialNL <= t;        
+            // Can only send NL after sending a Sync to someone
+        assert l'.globals.nextSerialNL <= l'.globals.nextSerialSync;
+            // At most f of such state transitions
+        assert l'.globals.procEpCount <= t;
+        assert l'.globals.prepCount <= t;
+        assert Sync_Serial_Invariant(tls');
+        i := i + 1;
+    }
+}
+
+predicate Quorums_Size_Invariant(tls:TLS_State) {
+    var n := |tls.config|;
+    forall ep | ep in tls.t_servers && tls.t_servers[ep].v.LeaderPeer? :: (
+        // && var ld := tls.t_servers[ep].v.leader;
+        && {tls.t_servers[ep].v.leader.my_id} <= tls.t_servers[ep].v.leader.globals.connectingFollowers
+        && {tls.t_servers[ep].v.leader.my_id} <= tls.t_servers[ep].v.leader.globals.electingFollowers
+        && {tls.t_servers[ep].v.leader.my_id} <= tls.t_servers[ep].v.leader.globals.ackSet
+        && 1 <= |tls.t_servers[ep].v.leader.globals.connectingFollowers| <= tls.f + 1
+        && 1 <= |tls.t_servers[ep].v.leader.globals.electingFollowers| <= tls.f + 1
+        && 1 <=|tls.t_servers[ep].v.leader.globals.ackSet| <= tls.f + 1
+    )
+}
+
+
+lemma lemma_Quorums_Size_Invariant_Proof(config:Config, tlb:seq<TLS_State>, t:int)
+    requires SeqIsUnique(config);
+    requires ValidTLSBehavior(config, tlb, t)
+    requires forall i | 0 <= i < |tlb| :: DS_Config_Invariant(config, tlb[i])
+    requires forall i | 0 <= i < |tlb| :: ZK_Config_Invariant(config, tlb[i])
+    ensures forall i | 0 <= i < |tlb| :: Quorums_Size_Invariant(tlb[i])
+{
+    assert Quorums_Size_Invariant(tlb[0]);
+    var i := 0;
+    while i < |tlb| - 1 
+        decreases |tlb| - i
+        invariant 0 <= i < |tlb|
+        invariant forall k | 0 <= k <= i :: Quorums_Size_Invariant(tlb[k])
+    {
+        var tls, tls' := tlb[i], tlb[i+1];
+        var actor, tios:seq<TZKIo> :| actor in tls.t_servers && TLS_NextOneServer(tls, tls', actor, tios);
+        if tls.t_servers[actor].v.LeaderPeer? {
+            var s, s', ios := tls.t_servers[actor].v.leader, tls'.t_servers[actor].v.leader, UntagLIoOpSeq(tios);
+            assert Quorums_Size_Invariant(tls');
+        }
+        i := i + 1;
+    }
+}
+
+
+
+predicate Follower_Serials_In_PreSync_Invariant(tls:TLS_State) 
+    requires |tls.config| > 0
+    requires tls.config[0] in tls.t_servers
+{
+    forall ep | 
+    && ep in tls.t_servers 
+    && tls.t_servers[ep].v.FollowerPeer? 
+    && tls.t_servers[ep].v.follower.state == F_PRESYNC
+    :: 
+    && var f := tls.t_servers[ep].v.follower;
+    && f.serialLI >= 0 
+    && f.serialSync < 0 
+    && f.serialNL < 0
+}
+
+predicate Follower_Serials_In_PreSync_Invariant_Helper(tls:TLS_State) 
+    requires |tls.config| > 0
+    requires tls.config[0] in tls.t_servers
+{
+    Follower_Serials_In_PreSync_Invariant(tls)
+    && forall ep | 
+    && ep in tls.t_servers 
+    && tls.t_servers[ep].v.FollowerPeer? 
+    && (|| tls.t_servers[ep].v.follower.state == F_HANDSHAKE_A
+        || tls.t_servers[ep].v.follower.state == F_HANDSHAKE_B)
+    ::
+    && var f := tls.t_servers[ep].v.follower;
+    && f.serialLI < 0 
+    && f.serialSync < 0 
+    && f.serialNL < 0
+}
+
+
+lemma lemma_Follower_Serials_In_PreSync_Invariant_Proof(config:Config, tlb:seq<TLS_State>, t:int)
+    requires SeqIsUnique(config);
+    requires ValidTLSBehavior(config, tlb, t)
+    requires forall i | 0 <= i < |tlb| :: DS_Config_Invariant(config, tlb[i])
+    requires forall i | 0 <= i < |tlb| :: ZK_Config_Invariant(config, tlb[i])
+    requires forall i | 0 <= i < |tlb| :: Quorums_Size_Invariant(tlb[i])
+    requires forall i | 0 <= i < |tlb| :: Handshake_Serial_Invariant(tlb[i])
+    ensures forall i | 0 <= i < |tlb| :: Follower_Serials_In_PreSync_Invariant_Helper(tlb[i])
+    ensures forall i | 0 <= i < |tlb| :: Follower_Serials_In_PreSync_Invariant(tlb[i])
+{
+    assert Follower_Serials_In_PreSync_Invariant_Helper(tlb[0]);
+    var i := 0;
+    while i < |tlb| - 1 
+        decreases |tlb| - i
+        invariant 0 <= i < |tlb|
+        invariant forall k | 0 <= k <= i :: Follower_Serials_In_PreSync_Invariant_Helper(tlb[k])
+    {   
+        var tls, tls' := tlb[i], tlb[i+1];
+        assert Follower_Serials_In_PreSync_Invariant_Helper(tls');
+        i := i + 1;
+    }
+}
+
+
+
+predicate Follower_Cannot_Receive_NewLeader_Before_Sync(tls:TLS_State) {
+    forall ep | ep in tls.t_servers && tls.t_servers[ep].v.FollowerPeer? 
+    :: 
+    && var f := tls.t_servers[ep].v.follower;
+    && (f.serialNL >= 0 ==> f.serialSync >= 0)
+    && (f.serialSync >= 0 ==> f.serialLI >= 0)
+    // Contrapos: If any of serialLI or serialSync are < 0, then f.serialNL < 0;
+}
+
+
+lemma lemma_Follower_Cannot_Receive_NewLeader_Before_Sync_Proof(config:Config, tlb:seq<TLS_State>, t:int)
+    requires SeqIsUnique(config);
+    requires ValidTLSBehavior(config, tlb, t)
+    requires forall i | 0 <= i < |tlb| :: DS_Config_Invariant(config, tlb[i])
+    requires forall i | 0 <= i < |tlb| :: ZK_Config_Invariant(config, tlb[i])
+    requires forall i | 0 <= i < |tlb| :: Handshake_Serial_Invariant(tlb[i])
+    requires forall i | 0 <= i < |tlb| :: Sync_Serial_Invariant(tlb[i])
+    ensures forall i | 0 <= i < |tlb| :: Follower_Cannot_Receive_NewLeader_Before_Sync(tlb[i])
+{
+    assert Follower_Cannot_Receive_NewLeader_Before_Sync(tlb[0]);
+    var i := 0;
+    while i < |tlb| - 1 
+        decreases |tlb| - i
+        invariant 0 <= i < |tlb|
+        invariant forall k | 0 <= k <= i :: Follower_Cannot_Receive_NewLeader_Before_Sync(tlb[k])
+    {   
+        var tls, tls' := tlb[i], tlb[i+1];
+        assert Follower_Cannot_Receive_NewLeader_Before_Sync(tls');
+        i := i + 1;
+    }
+}
+
+
+
+predicate Leader_Cannot_Receive_Ack_Before_Sending_All_Syncs_Invariant(tls:TLS_State) 
+    requires |tls.config| > 0
+    requires tls.config[0] in tls.t_servers
+    requires tls.t_servers[tls.config[0]].v.LeaderPeer?
+{
+    var l := tls.t_servers[tls.config[0]].v.leader;
+    (exists fid :: 
+        && fid in l.handlers 
+        && (l.handlers[fid].state == LH_PREP_SYNC || l.handlers[fid].state == LH_SYNC)
+    )
+    ==> 
+    |l.globals.ackSet| == 1
+}
+
+
+// ASSUMPTION: Sends take priority over receives
+lemma lemma_Leader_Cannot_Receive_Ack_Before_Sending_All_Syncs_Invariant_Proof(config:Config, tlb:seq<TLS_State>, f:int)
+    requires SeqIsUnique(config);
+    requires ValidTLSBehavior(config, tlb, f)
+    requires forall i | 0 <= i < |tlb| :: DS_Config_Invariant(config, tlb[i])
+    requires forall i | 0 <= i < |tlb| :: ZK_Config_Invariant(config, tlb[i])
+    ensures forall i | 0 <= i < |tlb| :: Leader_Cannot_Receive_Ack_Before_Sending_All_Syncs_Invariant(tlb[i]) 
+{
+    assert Leader_Cannot_Receive_Ack_Before_Sending_All_Syncs_Invariant(tlb[0]);
+    var i := 0;
+    while i < |tlb| - 1 
+        decreases |tlb| - i
+        invariant 0 <= i < |tlb|
+        invariant forall k | 0 <= k <= i :: Leader_Cannot_Receive_Ack_Before_Sending_All_Syncs_Invariant(tlb[k])
+    {
+        var tls, tls' := tlb[i], tlb[i+1];
+        assume false;
+        assert Leader_Cannot_Receive_Ack_Before_Sending_All_Syncs_Invariant(tls');
+        i := i + 1;
+    }
+}
+
+
+
+predicate Leader_Sends_All_LI_Before_Receiving_EpochAck_Invariant(tls:TLS_State) {
+    forall ep | ep in tls.t_servers && tls.t_servers[ep].v.LeaderPeer? :: (
+        && var leader := tls.t_servers[ep].v.leader;
+        && (
+            && |leader.globals.electingFollowers| > 1
+            ==> 
+            leader.globals.nextSerialLI == tls.f
+        )
+    )
+}
+
+// ASSUMPTION: Sends take priority over receives
+lemma lemma_Leader_Sends_All_LI_Before_Receiving_EpochAck_Invariant_Proof(config:Config, tlb:seq<TLS_State>, f:int)
+    requires SeqIsUnique(config);
+    requires ValidTLSBehavior(config, tlb, f)
+    requires forall i | 0 <= i < |tlb| :: DS_Config_Invariant(config, tlb[i])
+    requires forall i | 0 <= i < |tlb| :: ZK_Config_Invariant(config, tlb[i])
+    ensures forall i | 0 <= i < |tlb| :: Leader_Sends_All_LI_Before_Receiving_EpochAck_Invariant(tlb[i]) 
+{
+    assert Leader_Sends_All_LI_Before_Receiving_EpochAck_Invariant(tlb[0]);
+    var i := 0;
+    while i < |tlb| - 1 
+        decreases |tlb| - i
+        invariant 0 <= i < |tlb|
+        invariant forall k | 0 <= k <= i :: Leader_Sends_All_LI_Before_Receiving_EpochAck_Invariant(tlb[k])
+    {
+        var tls, tls' := tlb[i], tlb[i+1];
+        assume false;
+        assert Leader_Sends_All_LI_Before_Receiving_EpochAck_Invariant(tls');
+        i := i + 1;
+    }
+}
+
+
+
+}
