ironfleet/src/Dafny/Distributed/Protocol/ZooKeeper/PerformamceProof/TimestampedLS.dfy
@@ -1,0 +1,175 @@
+include "../../../Impl/Common/SeqIsUniqueDef.i.dfy"
+include "../../../Common/Framework/EnvironmentTCP.s.dfy"
+include "../Timestamps/TimestampedType.dfy"
+
+include "../Types.dfy"
+include "../DistributedSystem.dfy"
+include "../ZKEnvironment.dfy"
+include "../ZKDatabase.dfy"
+include "../Follower.dfy"
+include "../Leader.dfy"
+include "../LearnerHandler_Bug.dfy"
+include "Definitions.dfy"
+
+
+module ZooKeeper_TimestampedDistributedSystem {
+import opened Common__SeqIsUniqueDef_i
+import opened ZKTimestamp
+import opened ZooKeeper_Types
+import opened ZooKeeper_Environment
+import opened ZooKeeper_DistributedSystem
+import opened EnvironmentTCP_s
+import opened ZooKeeper_ZKDatabase
+import opened ZooKeeper_Follower
+import opened ZooKeeper_Leader
+import opened ZooKeeper_LearnerHandler
+import opened Zookeeper_Performance_Definitions
+
+type TQuorumPeer = TimestampedType<QuorumPeer>
+
+type TZKEnvironment = TimestampedLEnvironment<EndPoint, ZKMessage>
+
+type TZKIo = TimestampedLIoOp<EndPoint, ZKMessage>
+
+datatype TLS_State = TLS_State(
+    config:Config,
+    f:int,
+    t_environment: TZKEnvironment,
+    initialZkdbState: seq<ZKDatabase>,
+    t_servers: map<EndPoint, TQuorumPeer>
+)
+
+
+
+predicate TLS_Init(config:Config, tls:TLS_State, f: int) {
+    && f >= 1
+    && tls.f == f
+    && LS_Init(config, UntagLS_State(tls), f)
+    && tls.config == config
+    && |config| == f*2 + 1
+    && LEnvironment_Init(config, tls.t_environment)
+    && forall id | id in tls.t_servers :: tls.t_servers[id].ts == tls.t_servers[id].dts == TimeZero()
+}
+
+
+predicate TLS_NextOneServer(tls:TLS_State, tls':TLS_State, id:EndPoint, ios:seq<TZKIo>)
+        requires id in tls.t_servers;
+{
+    && LS_NextOneServer(UntagLS_State(tls), UntagLS_State(tls'), id, UntagLIoOpSeq(ios))
+    && tls.t_environment.nextStep == LEnvStepHostIos(id, ios)
+    && (forall t_io | t_io in ios && t_io.LIoOpSend? :: t_io.s.msg.ts == TimeAdd2(tls'.t_servers[id].ts, D))
+    && tls'.t_servers == tls.t_servers[id := tls'.t_servers[id]]
+    && var hs := ActionToHostStep(tls, tls', id, ios);
+
+    && (if |ios| > 0 && ios[0].LIoOpReceive? then   // Note that in performal, at most one rcv in each step
+            && tls'.t_servers[id].ts == TLS_RecvPerfUpdate(tls.t_servers[id].ts, ios[0].r.msg.ts, hs)
+            && tls'.t_servers[id].dts == ios[0].r.msg.ts
+            && tls.t_servers[id].dts <= ios[0].r.msg.ts  // (ARRIVAL-TIME) rule
+            // && tls.t_servers[id].dts <= ios[0].r.msg.ts <= tls.t_servers[id].ts + Timeout() // (ARRIVAL-TIME) rule
+        else
+            && tls'.t_servers[id].ts == TLS_NoRecvPerfUpdate(tls.t_servers[id].ts, hs)
+            && tls'.t_servers[id].dts == tls.t_servers[id].dts
+    )
+}
+
+
+predicate TLS_Next(tls:TLS_State, tls':TLS_State){
+        && LS_Next(UntagLS_State(tls), UntagLS_State(tls'))
+        && tls'.config == tls.config
+        && tls'.f == tls.f
+        && LEnvironment_Next(tls.t_environment, tls'.t_environment)
+        && (exists ep, ios :: ep in tls.t_servers && TLS_NextOneServer(tls, tls', ep, ios))
+}
+
+
+predicate ValidTLSBehavior(config:Config, tlb:seq<TLS_State>, f: int)  {
+    && |tlb| > 0
+    && TLS_Init(config, tlb[0], f)
+    && (forall i :: 0 <= i < |tlb| -1 ==> TLS_Next(tlb[i], tlb[i+1]))
+}
+
+
+
+/*****************************************************************************************
+*                                       Hoststep                                         *
+*****************************************************************************************/
+
+function ActionToHostStep(tls:TLS_State, tls':TLS_State, id:EndPoint, ios:seq<TZKIo>) : HostStep
+    requires id in tls.t_servers    
+    requires LS_NextOneServer(UntagLS_State(tls), UntagLS_State(tls'), id, UntagLIoOpSeq(ios))
+{
+    var ls, ls', zkios := UntagLS_State(tls), UntagLS_State(tls'), UntagLIoOpSeq(ios);
+    match ls.servers[id] 
+    case LeaderPeer(leader) => (
+        match leader.state
+        case L_RUNNING => L(LStutter)
+        case L_STARTING => (
+            var s, s' := ls.servers[id].leader, ls'.servers[id].leader;
+            if IsVerifiedQuorum(leader.my_id, |leader.globals.config|, leader.globals.ackSet) 
+            then L(LStutter)
+            else (
+                if IsVerifiedQuorum(s.my_id, |s.globals.config|, s.globals.ackSet) then L(LStutter) else
+                assert exists follower_id :: LHNext(s, s', follower_id, zkios);
+                var follower_id :| LHNext(s, s', follower_id, zkios);
+                match s.handlers[follower_id].state
+                case LH_HANDSHAKE_A => L(ProcessFollowerInfo)
+                case LH_HANDSHAKE_B => L(ProcessEpochAck)
+                case LH_PREP_SYNC => L(PrepSync)
+                case LH_SYNC => (
+                    if zkios[0].s.msg.SyncSNAP?
+                    then L(DoSyncSNAP)  // Sending a snapshot is a special event
+                    else L(DoSync)
+                )
+                case LH_PROCESS_ACK => 
+                    if s.globals.zkdb.isRunning then L(LStutter) else L(ProcessAck)
+                case LH_RUNNING => L(LStutter)
+                case LH_ERROR => L(LStutter)
+            )   
+        )
+    )
+    case FollowerPeer(follower) => (
+        match follower.state 
+        case F_HANDSHAKE_A => F(SendFollowerInfo)
+        case F_HANDSHAKE_B => F(ProcessLeaderInfo)
+        case F_PRESYNC => (
+            if zkios[0].r.msg.SyncSNAP? 
+                then F(ProcessSnap)   // Processing a snapshot is a special event
+            else if zkios[0].r.msg.SyncDIFF? || zkios[0].r.msg.SyncTRUNC? 
+                then F(ProcessSyncInfo)
+            else F(FStutter)
+        )
+        case F_SYNC => (
+            var s, s' := ls.servers[id].follower, ls'.servers[id].follower;
+            assert SyncWithLeader(s, s', zkios);
+            if zkios[0].r.msg.Commit? || zkios[0].r.msg.NewLeader? || zkios[0].r.msg.UpToDate?
+                then F(ProcessSync) 
+            else F(FStutter)
+        )
+        case F_RUNNING => F(FStutter)
+        case F_ERROR => F(FStutter)
+    )
+}
+
+
+
+/*****************************************************************************************
+*                                       Utilities                                        *
+*****************************************************************************************/
+
+function UntagLSServers(t_servers: map<EndPoint, TQuorumPeer>) : map<EndPoint, QuorumPeer>
+    ensures forall id :: id in t_servers <==> id in UntagLSServers(t_servers);
+    ensures forall id | id in t_servers :: UntagLSServers(t_servers)[id] == t_servers[id].v;
+{
+    map id | id in t_servers :: t_servers[id].v
+}
+
+function UntagLS_State(tds:TLS_State) : LS_State
+    ensures UntagLS_State(tds).servers == UntagLSServers(tds.t_servers);
+    ensures UntagLS_State(tds).environment == UntagLEnvironment(tds.t_environment);
+{
+    LS_State(
+        UntagLEnvironment(tds.t_environment),
+        tds.initialZkdbState,
+        UntagLSServers(tds.t_servers))
+}
+}
