ironfleet/src/Dafny/Distributed/Protocol/ZooKeeper/Types.dfy
@@ -1,0 +1,39 @@
+include "../../Common/Native/NativeTypes.s.dfy"
+include "../../Common/Framework/EnvironmentTCP.s.dfy"
+
+module ZooKeeper_Types {
+import opened Native__NativeTypes_s
+import opened EnvironmentTCP_s
+
+
+/*****************************************************************************************
+*                                       Hoststep                                         *
+*****************************************************************************************/
+
+datatype FollowerStep = 
+    SendFollowerInfo | ProcessLeaderInfo | ProcessSync | ProcessSyncInfo | ProcessSnap | FStutter
+
+datatype LeaderStep = 
+    ProcessFollowerInfo | ProcessEpochAck | PrepSync | DoSync | DoSyncSNAP | ProcessAck | LStutter
+
+
+datatype ZKStep = F(fs: FollowerStep) | L(ls:LeaderStep)
+
+
+/*****************************************************************************************
+*                                         ZXID                                           *
+*****************************************************************************************/
+
+datatype Zxid = Zxid(epoch:int, counter:int)
+
+const NullZxid := Zxid(-1, -1);
+
+predicate ZxidLt(z1:Zxid, z2:Zxid) {
+    if z1.epoch < z2.epoch then true
+    else z1.epoch == z2.epoch && z1.counter < z2.counter 
+}
+
+predicate ZxidEq(z1:Zxid, z2:Zxid) {
+    z1.epoch == z2.epoch && z1.counter == z2.counter 
+}
+}
