ironfleet/src/Dafny/Distributed/Protocol/ZooKeeper/ZKEnvironment.dfy
@@ -1,0 +1,34 @@
+include "../../Common/Native/NativeTypes.s.dfy"
+include "../../Common/Framework/EnvironmentTCP.s.dfy"
+include "ZKDatabase.dfy"
+include "Types.dfy"
+
+module ZooKeeper_Environment {
+import opened Native__NativeTypes_s
+import opened EnvironmentTCP_s
+import opened ZooKeeper_ZKDatabase
+import opened ZooKeeper_Types
+
+
+datatype EndPoint = EndPoint(addr:seq<byte>, port:uint16)
+    // UdpPacket_ctor has silly name to ferret out backwards calls
+
+type Config = seq<EndPoint>
+
+datatype ZKMessage = 
+    | FollowerInfo(sid:nat, latestZxid:Zxid)
+    | LeaderInfo(sid:nat, serial:nat, newZxid:Zxid)
+    | AckEpoch(sid:nat, serial:nat, lastLoggedZxid:Zxid, lastAcceptedEpoch:int)
+    | SyncDIFF(sid:nat, serial:nat, lastProcessedZxid:Zxid)
+    | SyncSNAP(sid:nat, serial:nat, leaderDb: ZKDatabase, lastProcessedZxid:Zxid)
+    | SyncTRUNC(sid:nat, serial:nat, lastProcessedZxid:Zxid)
+    | NewLeader(sid:nat, serial:nat, newLeaderZxid:Zxid)
+    | Commit(sid:nat, serial:nat, txn:Zxid)
+    | Ack(sid:nat, serial:nat, ackZxid:Zxid)
+    | UpToDate(sid:nat)
+
+type ZKEnvironment = LEnvironment<EndPoint, ZKMessage>
+type ZKPacket = LPacket<EndPoint, ZKMessage>
+type ZKIo = LIoOp<EndPoint, ZKMessage>
+
+}
